WIP classifiers overhaul
Make Kinds a flat list, might be able to progress

Capless/Classifier.lean
@@ -1,1051 +1,424 @@
-import Capless.Basic
-import Capless.Tactics
+import Capless.Classifier.Core
+import Capless.Classifier.Kind
+import Capless.Classifier.Intersection
+import Capless.Classifier.Subtract
+import Capless.Classifier.Subkind
 
 namespace Capless
 
-inductive Classifier : Type where
-  | top : Classifier
-  | child : Nat -> Classifier -> Classifier
-deriving DecidableEq
+-- inductive Kind.Disjoint : Kind -> Kind -> Prop where
+--   | empty_l: Disjoint .empty K
+--   | empty_r : Disjoint K .empty
+--   | union_l : Disjoint K1 K -> Disjoint K2 K -> Disjoint (K1.union K2) K
+--   | union_r : Disjoint K K1 -> Disjoint K K2 -> Disjoint K (K1.union K2)
+--   | absurd_l : ContainsSupOf ex1 r1 -> Disjoint (.node r1 ex1) (.node r2 ex2)
+--   | absurd_r : ContainsSupOf ex2 r2 -> Disjoint (.node r1 ex1) (.node r2 ex2)
+--   | root : r1.Disjoint r2 -> Disjoint (.node r1 ex1) (.node r2 ex2)
+--   | excl_l : ContainsSupOf ex2 r1 -> Disjoint (.node r1 ex1) (.node r2 ex2)
+--   | excl_r : ContainsSupOf ex1 r2 -> Disjoint (.node r1 ex1) (.node r2 ex2)
+
+-- theorem Kind.Disjoint.union_l_inv (hd : Disjoint (K1.union K2) K) : Disjoint K1 K ∧ Disjoint K2 K := by
+--   generalize hk : Kind.union K1 K2 = K' at hd
+--   induction hd with
+--   | empty_l => cases hk
+--   | empty_r => exact ⟨.empty_r, .empty_r⟩
+--   | union_l hd1 hd2 =>
+--     cases hk
+--     exact ⟨hd1, hd2⟩
+--   | union_r hd1 hd2 ih1 ih2 =>
+--     have ⟨hd1', hd2'⟩ := ih1 hk
+--     have ⟨hd1'', hd2''⟩ := ih2 hk
+--     exact ⟨.union_r hd1' hd1'', .union_r hd2' hd2''⟩
+--   | absurd_l => cases hk
+--   | absurd_r => cases hk
+--   | root => cases hk
+--   | excl_l => cases hk
+--   | excl_r => cases hk
+
+-- theorem Kind.Disjoint.union_r_inv (hd : Disjoint K (K1.union K2)) : Disjoint K K1 ∧ Disjoint K K2 := by
+--   generalize hk : Kind.union K1 K2 = K' at hd
+--   induction hd with
+--   | empty_l => exact ⟨.empty_l, .empty_l⟩
+--   | empty_r => cases hk
+--   | union_l hd1 hd2 ih1 ih2 =>
+--     have ⟨hd1', hd2'⟩ := ih1 hk
+--     have ⟨hd1'', hd2''⟩ := ih2 hk
+--     exact ⟨.union_l hd1' hd1'', .union_l hd2' hd2''⟩
+--   | union_r hd1 hd2 =>
+--     cases hk
+--     exact ⟨hd1, hd2⟩
+--   | absurd_l => cases hk
+--   | absurd_r => cases hk
+--   | root => cases hk
+--   | excl_l => cases hk
+--   | excl_r => cases hk
+
+-- theorem Kind.Disjoint.implies_empty_intersect (hd : K1.Disjoint K2) (hi : Intersect K1 K2 R) : IsEmpty R := by
+--   induction hi with
+--   | empty_l => exact .empty
+--   | empty_r => exact .empty
+--   | union_l hi1 hi2 ih1 ih2 =>
+--     have ⟨hd1, hd2⟩ := hd.union_l_inv
+--     exact .union (ih1 hd1) (ih2 hd2)
+--   | union_r hi1 hi2 ih1 ih2 =>
+--     have ⟨hd1, hd2⟩ := hd.union_r_inv
+--     exact .union (ih1 hd1) (ih2 hd2)
+--   | singleton_l hs =>
+--     cases hd with
+--     | absurd_l ha => exact .absurd (.append_l ha)
+--     | absurd_r ha => exact .absurd (.append_r (ha.trans_subclass hs))
+--     | root hd => cases hd.not_subclass hs
+--     | excl_l ha => exact .absurd (.append_r ha)
+--     | excl_r ha => exact .absurd (.append_l (ha.trans_subclass hs))
+--   | singleton_r hs =>
+--     cases hd with
+--     | absurd_l ha => exact .absurd (.append_l (ha.trans_subclass hs))
+--     | absurd_r ha => exact .absurd (.append_r ha)
+--     | root hd => cases hd.symm.not_subclass hs
+--     | excl_l ha => exact .absurd (.append_r (ha.trans_subclass hs))
+--     | excl_r ha => exact .absurd (.append_l ha)
+--   | singleton_disj => exact .empty
+
+-- theorem Kind.Disjoint.from_empty_intersect (hi : Intersect K1 K2 R) (he : IsEmpty R) : K1.Disjoint K2 := by
+--   induction hi with
+--   | empty_l => exact .empty_l
+--   | empty_r => exact .empty_r
+--   | union_l hi1 hi2 ih1 ih2 =>
+--     cases he with
+--     | union he1 he2 => exact .union_l (ih1 he1) (ih2 he2)
+--   | union_r hi1 hi2 ih1 ih2 =>
+--     cases he with
+--     | union he1 he2 => exact .union_r (ih1 he1) (ih2 he2)
+--   | singleton_l hs =>
+--     cases he with
+--     | absurd ha =>
+--       cases ha.of_append with
+--       | inl ha => exact .absurd_l ha
+--       | inr ha => exact .excl_l ha
+--   | singleton_r hs =>
+--     cases he with
+--     | absurd ha =>
+--       cases ha.of_append with
+--       | inl ha => exact .excl_r ha
+--       | inr ha => exact .absurd_r ha
+--   | singleton_disj hd => exact .root hd
+
+-- theorem Kind.Disjoint.top_l (hd: Disjoint .top K) : IsEmpty K := by
+--   cases hd
+--   case empty_r => constructor
+--   case union_r ha hb => apply IsEmpty.union ha.top_l hb.top_l
+--   case absurd_l hsc => cases hsc
+--   case absurd_r hsc => constructor; assumption
+--   case root hd => cases hd.symm.not_subclass .of_top
+--   case excl_l hsc => constructor; apply hsc.trans_subclass .of_top
+--   case excl_r hsc => cases hsc
+
+-- theorem Kind.Disjoint.symm (hd : K1.Disjoint K2) : Disjoint K2 K1 := by
+--   induction hd with
+--   | empty_l => exact .empty_r
+--   | empty_r => exact .empty_l
+--   | union_l _ _ ih1 ih2 => exact .union_r ih1 ih2
+--   | union_r _ _ ih1 ih2 => exact .union_l ih1 ih2
+--   | absurd_l ha => exact .absurd_r ha
+--   | absurd_r ha => exact .absurd_l ha
+--   | root hd => exact .root hd.symm
+--   | excl_l ha => exact .excl_r ha
+--   | excl_r ha => exact .excl_l ha
+
+-- theorem Kind.Disjoint.append_excl_l (hd : Disjoint (.node r1 ex2) K) : Disjoint (.node r1 (ex1 ++ ex2)) K := by
+--   cases hd
+--   case empty_r => apply! empty_r
+--   case union_r ha hb => apply union_r ha.append_excl_l hb.append_excl_l
+--   case absurd_l ha => apply absurd_l ha.append_r
+--   case absurd_r => apply! absurd_r
+--   case root => apply! root
+--   case excl_l => apply! excl_l
+--   case excl_r ha => apply excl_r ha.append_r
+
+-- theorem Kind.Disjoint.refine_subroot_l (hd : Disjoint (.node r1 ex1) K) (hs : r2.Subclass r1) : Disjoint (.node r2 ex1) K := by
+--   cases hd
+--   case empty_r => apply! empty_r
+--   case union_r ha hb => apply! union_r (ha.refine_subroot_l _) (hb.refine_subroot_l _)
+--   case absurd_l ha => apply! absurd_l $ ha.trans_subclass _
+--   case absurd_r => apply! absurd_r
+--   case root hdr => apply root; apply! hdr.refines_subclass_l _
+--   case excl_l hc => apply! excl_l $ hc.trans_subclass _
+--   case excl_r => apply! excl_r
+
+-- -- If K1 is disjoint from K', and R is the intersection of K with K1, then R is disjoint from K'
+-- theorem Kind.Disjoint.intersect_disjoint (hd : K1.Disjoint K') (hi : Intersect K K1 R) : R.Disjoint K' := by
+--   induction hi
+--   case empty_l => apply! empty_l
+--   case empty_r => apply! empty_l
+--   case union_l iha ihb => apply! union_l (iha _) (ihb _)
+--   case union_r iha ihb =>
+--     have ⟨_, _⟩ := hd.union_l_inv
+--     apply! union_l (iha _) (ihb _)
+--   case singleton_l hs => apply append_excl_l; apply! hd.refine_subroot_l _
+--   case singleton_r hs => apply hd.append_excl_l
+--   case singleton_disj hdr => apply empty_l
+
+-- theorem Kind.Disjoint.absurd_l' (hs : ContainsSupOf ex1 r1) : Disjoint (.node r1 ex1) K := by
+--   induction K
+--   case empty => apply empty_r
+--   case node => apply! absurd_l
+--   case union ha hb => apply! union_r
+
+-- theorem Kind.Disjoint.refine_subtract_l (hd : Disjoint K1 K) (hs : Subtract K1 K2 R) : Disjoint R K := by
+--   induction hs
+--   case empty_l => exact .empty_l
+--   case union_l ih1 ih2 =>
+--     have ⟨hd1, hd2⟩ := hd.union_l_inv
+--     exact .union_l (ih1 hd1) (ih2 hd2)
+--   case empty_r => assumption
+--   case union_r ih1 ih2 => exact ih2 (ih1 hd)
+--   case tree => apply! hd.append_excl_l (ex1 := [_])
+--   case excl_absurd_r => assumption
+--   case excl_irrelevant_r ih => apply! ih
+--   case excl_subclass_r hs1 _ ih =>
+--     apply Disjoint.union_l
+--     apply! ih
+--     apply! hd.refine_subroot_l
+--   case excl_subclass_l => assumption
+--   case excl_irrelevant_l ih => apply! ih
+
+-- theorem Kind.Disjoint.append_l_disj_inv (hd : Disjoint (.node r1 (a :: ex1)) (.node r2 ex2)) (hda : a.Disjoint r2) : Disjoint (.node r1 ex1) (.node r2 ex2) := by
+--   cases hd
+--   case absurd_l hsc =>
+--     cases hsc
+--     case here hs => apply! root $ hda.refines_subclass_l _
+--     case there hsc => apply! absurd_l
+--   case absurd_r => apply! absurd_r
+--   case root => apply! root
+--   case excl_l hsc => apply! excl_l
+--   case excl_r hsc =>
+--     cases hsc
+--     case here hs => cases hda.symm.not_subclass hs
+--     case there => apply! excl_r
+
+-- theorem Kind.Disjoint.append_l_contained_inv (hd : Disjoint (.node r1 (a :: ex1)) (.node r2 ex2)) (hsc: ContainsSupOf ex2 a) : Disjoint (.node r1 ex1) (.node r2 ex2) := by
+--   cases hd
+--   case absurd_l hsc =>
+--     cases hsc
+--     case here hs => apply! excl_l $ hsc.trans_subclass _
+--     case there hsc => apply! absurd_l
+--   case absurd_r => apply! absurd_r
+--   case root => apply! root
+--   case excl_l hsc => apply! excl_l
+--   case excl_r hsc =>
+--     cases hsc
+--     case here hs => apply! absurd_r $ hsc.trans_subclass _
+--     case there => apply! excl_r
+
+-- theorem Kind.Disjoint.refine_disjoint_subtract_l_disjoint_root
+--   (hdr : Disjoint R K)
+--   (hs : Subtract (.node r1 ex1) (.node r2 ex2) R)
+--   (hd : r1.Disjoint r2)
+--   : Disjoint (.node r1 ex1) K := by
+--   cases hs
+--   case tree =>
+--     generalize h : node r1 (r2 :: ex1) = L at hdr
+--     induction hdr <;> try cases h
+--     case empty_r => apply! empty_r
+--     case union_r ha hb => simp_all; apply! union_r
+--     case absurd_l hsc =>
+--       cases hsc
+--       case here hs => cases hd.not_subclass hs
+--       case there hsc => apply! absurd_l
+--     case absurd_r => apply! absurd_r
+--     case root hd2 => apply! root
+--     case excl_l => apply! excl_l
+--     case excl_r hsc =>
+--       cases hsc
+--       case here hs => apply! root $ hd.refines_subclass_r _
+--       case there hsc => apply! excl_r
+--   case excl_absurd_r => assumption
+--   case excl_irrelevant_r hs => apply! hdr.refine_disjoint_subtract_l_disjoint_root
+--   case excl_subclass_r hs =>
+--     have ⟨hl, _⟩ := hdr.union_l_inv
+--     apply! hl.refine_disjoint_subtract_l_disjoint_root _ hd
+--   case excl_subclass_l => assumption
+--   case excl_irrelevant_l hs => apply! hdr.refine_disjoint_subtract_l_disjoint_root
+
+-- theorem Kind.Disjoint.refine_disjoint_subtract_l_subroot
+--   (hdr : Disjoint R K)
+--   (hs : Subtract (.node r1 ex1) (.node r2 ex2) R)
+--   (hsub : r2.Subclass r1)
+--   (hd2 : Disjoint (.node r2 ex1) K)
+--   : Disjoint (.node r1 ex1) K := by
+--   cases hs
+--   case tree =>
+--     generalize h : node r1 (r2 :: ex1) = L at hdr
+--     induction hdr <;> try cases h
+--     case empty_r => apply! empty_r
+--     case union_r ha hb =>
+--       have ⟨_, _⟩ := hd2.union_r_inv
+--       simp_all
+--       apply! union_r
+--     case absurd_l hsc =>
+--       cases hsc
+--       case here hs2 => cases hsub.antisymm hs2; assumption
+--       case there => apply! absurd_l
+--     case absurd_r => apply! absurd_r
+--     case root => apply! root
+--     case excl_l => apply! excl_l
+--     case excl_r hsc =>
+--       cases hsc
+--       case here hs2 =>
+--         cases hd2
+--         case absurd_l => apply excl_r; apply! ContainsSupOf.trans_subclass
+--         case absurd_r => apply! absurd_r
+--         case root hd => cases hd.symm.not_subclass hs2
+--         case excl_l hsc => apply! absurd_r $ hsc.trans_subclass _
+--         case excl_r hsc => apply! excl_r
+--       case there hsc => apply! excl_r
+--   case excl_absurd_r => assumption
+--   case excl_irrelevant_r hs =>  apply! hdr.refine_disjoint_subtract_l_subroot
+--   case excl_subclass_r hs =>
+--     have ⟨hl, _⟩ := hdr.union_l_inv
+--     apply! hl.refine_disjoint_subtract_l_subroot
+--   case excl_subclass_l => assumption
+--   case excl_irrelevant_l hs => apply! hdr.refine_disjoint_subtract_l_subroot
+
+
+
+-- theorem Kind.Disjoint.refine_disjoint_subtract_l (hd2 : Disjoint K2 K) (hs : Subtract K1 K2 R) (hdr : Disjoint R K) : Disjoint K1 K := by
+--   induction hs generalizing K
+--   case empty_l => apply empty_l
+--   case union_l ih1 ih2 =>
+--     have ⟨_, _⟩ := hdr.union_l_inv
+--     apply! union_l (ih1 _ _) (ih2 _ _)
+--   case empty_r => assumption
+--   case union_r ha hb =>
+--     have ⟨hl, hr⟩ := hd2.union_l_inv
+--     apply ha hl _
+--     apply hb hr hdr
+--   case tree r1 ex1 r2 =>
+--     generalize h : node r1 (r2 :: ex1) = L at hdr
+--     induction hdr <;> try cases h
+--     case empty_r => apply! empty_r
+--     case union_r ha hb =>
+--       have ⟨_, _⟩ := hd2.union_r_inv
+--       simp_all
+--       apply! union_r
+--     case absurd_l hsc =>
+--       cases hsc
+--       case here hs =>
+--         cases hd2
+--         case absurd_l hsc => cases hsc
+--         case absurd_r hsc => apply! absurd_r
+--         case root hd =>  apply root; apply! hd.refines_subclass_l _
+--         case excl_l hsc => apply excl_l; apply! hsc.trans_subclass
+--         case excl_r hsc => cases hsc
+--       case there hsc => apply! absurd_l
+--     case absurd_r => apply! absurd_r
+--     case root => apply! root
+--     case excl_l => apply! excl_l
+--     case excl_r hsc =>
+--       cases hsc
+--       case here hs =>
+--         cases hd2
+--         case absurd_r hsc => apply! absurd_r
+--         case root hd => cases hd.symm.not_subclass hs
+--         case excl_l hsc => apply absurd_r; apply! hsc.trans_subclass
+--         case excl_r hsc => cases hsc
+--         case absurd_l hsc => cases hsc
+--       case there hsc => apply! excl_r
+--   case excl_subclass_r r1 ex1 r2 ex2 _ a hss hsc hs ih =>
+--     have ⟨hdr1, hdr2⟩ := hdr.union_l_inv
+--     generalize h : node r2 (a :: ex2) = L at hd2
+--     induction hd2 generalizing K2 <;> try cases h
+--     case empty_r => apply! empty_r
+--     case union_r ha hb =>
+--       simp_all
+--       have ⟨_, _⟩ := hdr.union_r_inv
+--       have ⟨_, _⟩ := hdr1.union_r_inv
+--       have ⟨_, _⟩ := hdr2.union_r_inv
+--       apply! union_r (ha _ _ _) (hb _ _ _)
+--     case absurd_l hsc =>
+--       cases hsc
+--       case here hsc1 =>
+--         cases hss.antisymm hsc1
+--         apply! hdr1.refine_disjoint_subtract_l_subroot
+--       case there hsc =>
+--         apply ih _ hdr1
+--         apply! absurd_l
+--     case absurd_r => apply! absurd_r
+--     case root hd1 => apply ih (.root hd1) hdr1
+--     case excl_l hsc => apply! ih (.excl_l _)
+--     case excl_r hsc =>
+--       cases hsc
+--       case here hs =>
+--         cases hdr2
+--         case absurd_l hsc => apply! excl_r $ hsc.trans_subclass _
+--         case absurd_r => apply! absurd_r
+--         case root hd => cases hd.symm.not_subclass hs
+--         case excl_l hsc => apply! absurd_r $ hsc.trans_subclass _
+--         case excl_r => apply! excl_r
+--       case there hsc => apply! ih (excl_r _)
+--   case excl_absurd_r hs => assumption
+--   case excl_irrelevant_r r1 ex1 r2 ex2 _ a hd hs ih =>
+--     generalize h : node r2 (a :: ex2) = L at hd2
+--     induction hd2 generalizing K2 <;> try cases h
+--     case empty_r => apply! empty_r
+--     case union_r ha hb =>
+--       simp_all
+--       have ⟨_, _⟩ := hdr.union_r_inv
+--       apply! union_r (ha _) (hb _)
+--     case absurd_l hsc =>
+--       cases hsc
+--       case here hsc => cases hd.not_subclass hsc
+--       case there hsc =>
+--         apply ih _ hdr
+--         apply! absurd_l
+--     case absurd_r => apply! absurd_r
+--     case root hd1 => apply ih (.root hd1) hdr
+--     case excl_l hsc => apply! ih (.excl_l _)
+--     case excl_r hsc =>
+--       cases hsc
+--       case here hs => apply ih _ hdr; apply root; apply! hd.refines_subclass_r
+--       case there hsc => apply! ih (excl_r _)
+--   case excl_subclass_l hs2 hs1 => assumption
+--   case excl_irrelevant_l r1 ex1 r2 ex2 _ a hs2 hd1 hs ih =>
+--     generalize h : node r2 (a :: ex2) = L at hd2
+--     induction hd2 generalizing K2 <;> try cases h
+--     case empty_r => apply! empty_r
+--     case union_r ha hb =>
+--       simp_all
+--       have ⟨_, _⟩ := hdr.union_r_inv
+--       apply! union_r (ha _) (hb _)
+--     case absurd_l hsc =>
+--       cases hsc
+--       case here hsc =>
+--         cases hs2.antisymm hsc
+--         apply! hdr.refine_disjoint_subtract_l_disjoint_root hs
+--       case there hsc =>
+--         apply ih _ hdr
+--         apply! absurd_l
+--     case absurd_r => apply! absurd_r
+--     case root hd1 => apply ih (.root hd1) hdr
+--     case excl_l hsc => apply! ih (.excl_l _)
+--     case excl_r hsc =>
+--       cases hsc
+--       case here hs => apply root; apply! hd1.refines_subclass_r
+--       case there hsc => apply! ih (excl_r _)
+
+-- theorem Kind.Disjoint.is_empty_l (he : IsEmpty K) : Disjoint K L := by
+--   induction he
+--   case empty => apply empty_l
+--   case absurd => apply! absurd_l'
+--   case union ha hb => apply! union_l
+
+-- theorem Kind.Disjoint.refine_subkind_l' (hd : Disjoint K2 K) (hs : Subtract K1 K2 R) (he : IsEmpty R) : Disjoint K1 K := by
+--   apply refine_disjoint_subtract_l hd hs
+--   apply is_empty_l he
+
+-- theorem Kind.Disjoint.refine_subkind_l (hd : Disjoint K2 K) (hs : Subkind K1 K2) : Disjoint K1 K := by
+--   cases hs
+--   apply! hd.refine_subkind_l'
+
+-- theorem Kind.Subkind.refine_disjoint_l (hs : Subkind K1 K2) (hd : Disjoint K2 K) : Disjoint K1 K := hd.refine_subkind_l hs
 
-def Classifier.control := child 0 .top
-
-inductive Classifier.Subclass : Classifier -> Classifier -> Prop where
-  | rfl : Subclass a a
-  | parent_l : Subclass a b -> Subclass (child n a) b
-
-inductive Classifier.StrictSub : Classifier -> Classifier -> Prop where
-  | child : StrictSub (child n a) a
-  | parent_l : StrictSub a b -> StrictSub (child n a) b
-
-theorem Classifier.Subclass.might_strict (hs : Subclass a b) : a = b ∨ StrictSub a b := by
-  induction hs
-  case rfl => left; simp
-  case parent_l hp ih =>
-    right
-    cases ih
-    case inl => subst_vars; constructor
-    case inr => apply! StrictSub.parent_l
-
-theorem Classifier.StrictSub.weaken (hs : StrictSub a b) : Subclass a b := by
-  induction hs
-  case child => apply Subclass.parent_l .rfl
-  case parent_l hp ih => apply Subclass.parent_l ih
-
-theorem Classifier.StrictSub.size (hs : StrictSub a b) : sizeOf a > sizeOf b := by induction hs <;> (simp; try omega)
-
-theorem Classifier.StrictSub.neq (hs : StrictSub a b) : a ≠ b := by
-  apply Ne.intro
-  intro h
-  have hs := hs.size
-  rw [h] at hs
-  omega
-
-inductive Classifier.Disjoint : Classifier -> Classifier -> Prop where
-  | base : n != m -> Disjoint (child n p) (child m p)
-  | left : Disjoint a b -> Disjoint (child n a) b
-  | right : Disjoint a b -> Disjoint a (child m b)
-
-theorem Classifier.Subclass.of_top : Subclass a .top := by
-  induction a
-  case top => apply rfl
-  case child n k ih => apply parent_l ih
-
-theorem Classifier.Subclass.parent_r (hs : Subclass a (child n b)) : Subclass a b := by
-  cases hs
-  case rfl => apply parent_l rfl
-  case parent_l hp =>
-    apply parent_l hp.parent_r
-
-theorem Classifier.Subclass.trans (h1 : Subclass a b) (h2 : Subclass b c) : Subclass a c := by
-  induction h2
-  case rfl => assumption
-  case parent_l hp ih => apply ih h1.parent_r
-
-theorem Classifier.Subclass.down_r (hs : Subclass a b) : a = b ∨ ∃ n, Subclass a (child n b) := by
-  induction hs
-  case rfl => simp
-  case parent_l ih =>
-    rename_i n _
-    right
-    cases ih
-    case inl ih => subst_vars; exists n; constructor
-    case inr ih =>
-      have ⟨m, ih⟩ := ih
-      exists m
-      apply parent_l ih
-
-theorem Classifier.Subclass.size (hs : Subclass a b) : sizeOf a ≥ sizeOf b := by
-  induction hs <;> (simp; try omega)
-
-theorem Classifier.Subclass.antisymm (h1 : Subclass a b) (h2 : Subclass b a) : a = b := by
-  induction h1
-  case rfl => simp
-  case parent_l hp ih =>
-    have hp1 := hp.size
-    have h21 := h2.size
-    simp at h21
-    omega
-
-theorem Classifier.StrictSub.antisymm (hs : StrictSub a b) (hs2 : Subclass b a) : False := by
-  have h := hs.size
-  have h2 := hs2.size
-  omega
-
-theorem Classifier.StrictSub.subclass_r (hss : StrictSub a b) (hs : Subclass b c) : StrictSub a c := by
-  induction hss
-  case child n a =>
-    induction hs generalizing n
-    case rfl => apply child
-    case parent_l m k ih =>
-      apply parent_l ih
-  case parent_l n a ih =>
-    apply! parent_l $ ih _
-
-theorem Classifier.Disjoint.symm (hd : Disjoint a b) : Disjoint b a := by
-  induction hd
-  case base hne =>
-    apply base; aesop
-  case left => apply! right
-  case right => apply! left
-
-theorem Classifier.Disjoint.refines_subclass_r
-  (hd : Disjoint b a2)
-  (hs : Subclass a1 a2) : Disjoint b a1 := by
-  induction hs
-  case rfl => assumption
-  case parent_l hs ih =>
-    apply right $ ih hd
-
-theorem Classifier.Disjoint.refines_subclass_l (hd : Disjoint a2 b) (hs : Subclass a1 a2) : Disjoint a1 b := by
-  apply symm
-  apply refines_subclass_r hd.symm hs
-
-theorem Classifier.Disjoint.left_inv (hd : Disjoint (child n a) b) : Subclass b a ∨ Disjoint a b := by
-  cases hd
-  case base m _ => left; constructor; constructor;
-  case left => right; assumption
-  case right hd =>
-    cases hd.left_inv
-    case inl hd => left; constructor; assumption
-    case inr hd => right; apply! right
-
-theorem Classifier.Disjoint.not_subclass (hd : Disjoint a b) (hs : Subclass a b) : False := by
-  induction a generalizing b
-  case top =>
-    induction b
-    case top => cases hd
-    case child n p ih => cases hs
-  case child n p ih =>
-    induction b
-    case top => cases hs; cases hd; apply! ih
-    case child m q ih2 =>
-      cases hs
-      case rfl =>
-        cases hd
-        case base => aesop
-        case left hs => apply ih2 hs.symm $ .parent_l .rfl
-        case right hs => apply ih2 hs $ .parent_l .rfl
-      case parent_l hs =>
-        cases hd
-        case base => have h := hs.size; simp at h; omega
-        case left => apply! ih
-        case right hd =>
-          cases hd.left_inv
-          case inl hd =>
-            have h := hs.parent_r.antisymm hd
-            subst_vars
-            have h := hs.size; simp at h; omega
-          case inr hd =>
-            apply ih (b:=q) hd hs.parent_r
-
-theorem Classifier.Disjoint.to_subclass (hd : Disjoint a b) (hs : Subclass c b) : Disjoint a c := by
-  induction hs
-  case rfl => assumption
-  case parent_l hp ih =>
-    apply right
-    apply ih hd
-
-theorem Classifier.subclass_or_disjoint a b:
-  Subclass a b ∨ StrictSub b a ∨ Disjoint a b := by
-  induction a
-  case top =>
-    cases Subclass.of_top (a:=b).might_strict
-    case inl => simp_all; left; exact .rfl
-    case inr => aesop
-  case child n k ih =>
-    cases ih
-    case inl ih =>
-      left; constructor; assumption
-    case inr ih =>
-      cases ih
-      case inl ih =>
-        cases ih.weaken.down_r
-        { subst_vars; left; apply Subclass.parent_l .rfl }
-        { rename_i ih1; have ⟨m, ih1⟩ := ih1;
-          generalize h : (n == m) = h0;
-          cases h0
-          right; right;
-          apply Disjoint.refines_subclass_r; apply Disjoint.base (m:=m); aesop; assumption
-          have h0 := LawfulBEq.eq_of_beq h; subst_vars
-          cases ih1.might_strict
-          . left; subst_vars; exact .rfl
-          . aesop
-        }
-      case inr ih =>
-        right; right; apply Disjoint.left ih
-
-def Classifier.subclass (a : Classifier) (b : Classifier) :=
-  if a == b then true
-  else match a with
-    | .top => false
-    | .child n p => p.subclass b
-
-theorem Classifier.subclass_is_Subclass : Subclass a b ↔ a.subclass b := by
-  apply Iff.intro
-  . intro hs
-    induction hs
-    case rfl => unfold subclass; simp
-    case parent_l n p => unfold subclass; simp; right; assumption
-  . intro hs
-    unfold subclass at hs
-    split at hs
-    case isTrue h =>
-      have h1 := LawfulBEq.eq_of_beq h
-      subst_vars
-      constructor
-    case isFalse h =>
-      split at hs
-      . contradiction
-      . rename_i p
-        constructor
-        rw [subclass_is_Subclass (a:=p)]
-        assumption
-
-def Classifier.disjoint (a : Classifier) (b : Classifier) :=
-  match a with
-  | .top => false
-  | .child n p =>
-    match b with
-    | .top => false
-    | .child m q =>
-      if p == q then n != m
-      else disjoint (.child n p) q || disjoint p (.child m q)
-
-theorem Classifier.disjoint_is_Disjoint {a b : Classifier} : Disjoint a b ↔ a.disjoint b := by
-  apply Iff.intro
-  . intro hs
-    induction hs with
-    | base hne =>
-      unfold disjoint
-      simp [hne]
-    | @left a' b' n ha ih =>
-      unfold disjoint
-      match b' with
-      | .top => cases ha.not_subclass .of_top
-      | .child m q =>
-        simp only
-        split
-        . rename_i heq
-          have h1 := LawfulBEq.eq_of_beq heq
-          subst_vars
-          cases ha.symm.not_subclass $ .parent_l .rfl
-        . simp [ih]
-    | @right a' b' m ha ih =>
-      unfold disjoint
-      match a' with
-      | .top =>
-        have : ∀ c, ¬ Disjoint top c := fun c h => by
-          induction c with
-          | top => cases h
-          | child n p ih =>
-            cases h with
-            | right ha => exact ih ha
-        exact absurd ha (this _)
-      | .child n p =>
-        simp only
-        split
-        . rename_i heq
-          have heq' := LawfulBEq.eq_of_beq heq
-          subst heq'
-          cases ha.not_subclass $ .parent_l .rfl
-        . simp [ih]
-  . intro hs
-    unfold disjoint at hs
-    split at hs
-    . cases hs
-    . split at hs
-      . cases hs
-      . split at hs
-        . rename_i h
-          have h1 := LawfulBEq.eq_of_beq h
-          subst_vars
-          apply! Disjoint.base
-        . simp at hs
-          cases hs
-          case inl hs =>
-            apply Disjoint.right
-            rw [disjoint_is_Disjoint]
-            assumption
-          case inr hs =>
-            apply Disjoint.left
-            rw [disjoint_is_Disjoint]
-            assumption
-termination_by sizeOf a + sizeOf b
-
--- **
--- Kinds
--- **
-
-inductive Kind : Type where
-  | empty : Kind
-  | node : Classifier -> List Classifier -> Kind -- .only[K].except[K1, ..., Kn]
-  | union : Kind -> Kind -> Kind
-
-@[simp]
-def Kind.top := node .top []
-
--- Shorthand notation for a subtree without exclusions
-@[simp]
-def Kind.classifier c := node c []
-
-def Kind.sup (a: Kind) (b: Kind) : Kind := a.union b
-
-def Kind.inf (a: Kind) (b: Kind) : Kind :=
-  match a with
-  | .empty => b
-  | .union a1 a2 => union (a1.inf b) (a2.inf b)
-  | .node r1 ex1 =>
-    match b with
-    | .empty => .empty
-    | .union b1 b2 => union (inf (.node r1 ex1) b1) (inf (.node r1 ex1) b2)
-    | .node r2 ex2 =>
-      if r1.subclass r2 then .node r1 (ex1 ++ ex2)
-      else if r2.subclass r1 then .node r2 (ex1 ++ ex2)
-      else .empty
-
-inductive ContainsSupOf : List Classifier -> Classifier -> Prop where
-  | here : b.Subclass a -> ContainsSupOf (a :: xs) b
-  | there : ContainsSupOf xs b -> ContainsSupOf (a :: xs) b
-
-theorem ContainsSupOf.append_l (h : ContainsSupOf xs b) : ContainsSupOf (xs ++ ys) b := by
-  induction h with
-  | here hs => exact .here hs
-  | there _ ih => exact .there ih
-
-theorem ContainsSupOf.append_r (h : ContainsSupOf ys b) : ContainsSupOf (xs ++ ys) b := by
-  induction xs with
-  | nil => exact h
-  | cons _ _ ih => exact .there ih
-
-theorem ContainsSupOf.trans_subclass (h : ContainsSupOf xs a) (hs : b.Subclass a) : ContainsSupOf xs b := by
-  induction h with
-  | here hs' => exact .here (hs.trans hs')
-  | there _ ih => exact .there (ih hs)
-
-theorem ContainsSupOf.of_append (h : ContainsSupOf (xs ++ ys) b) : ContainsSupOf xs b ∨ ContainsSupOf ys b := by
-  induction xs with
-  | nil => exact .inr h
-  | cons a xs ih =>
-    cases h with
-    | here hs => exact .inl (.here hs)
-    | there h =>
-      cases ih h with
-      | inl h => exact .inl (.there h)
-      | inr h => exact .inr h
-
-inductive Kind.IsEmpty : Kind -> Prop where
-  | empty : IsEmpty .empty
-  | absurd : ContainsSupOf exs r -> IsEmpty (.node r exs)
-  | union : IsEmpty K1 -> IsEmpty K2 -> IsEmpty (.union K1 K2)
-
-theorem Kind.IsEmpty.is_absurd (he : IsEmpty (.node r exs)) : ContainsSupOf exs r := by
-  cases he; assumption
-
-inductive Kind.Intersect : Kind -> Kind -> Kind -> Prop where
-  | empty_l : Intersect .empty K .empty
-  | empty_r : Intersect K .empty .empty
-  | union_l : Intersect K1 K R1 -> Intersect K2 K R2 -> Intersect (K1.union K2) K (R1.union R2)
-  | union_r : Intersect K K1 R1 -> Intersect K K2 R2 -> Intersect K (K1.union K2) (R1.union R2)
-  | singleton_l : r1.Subclass r2 -> Intersect (.node r1 ex1) (.node r2 ex2) (.node r1 (ex1 ++ ex2))
-  | singleton_r : r2.Subclass r1 -> Intersect (.node r1 ex1) (.node r2 ex2) (.node r2 (ex1 ++ ex2))
-  | singleton_disj : r1.Disjoint r2 -> Intersect (.node r1 ex1) (.node r2 ex2) .empty
-
-@[simp]
-def Kind.intersect (k : Kind) (l : Kind) : Kind :=
-  match k with
-  | .empty => .empty
-  | .union k1 k2 => .union (k1.intersect l) (k2.intersect l)
-  | .node r1 ex1 =>
-    match l with
-    | .empty => .empty
-    | .union l1 l2 => .union ((node r1 ex1).intersect l1) ((node r1 ex1).intersect l2)
-    | .node r2 ex2 =>
-      if r1.subclass r2 then .node r1 (ex1 ++ ex2)
-      else if r2.subclass r1 then .node r2 (ex1 ++ ex2)
-      else .empty
-
-theorem Kind.Intersect.lawful : Intersect K L (K.intersect L) := by
-  induction K generalizing L
-  case empty => unfold intersect; apply empty_l
-  case union ha hb =>
-    unfold intersect
-    apply union_l ha hb
-  case node r1 ex1 =>
-    induction L
-    case empty => unfold intersect; simp; apply empty_r
-    case union ha hb => unfold intersect; simp; apply union_r ha hb
-    case node r2 ex2 =>
-      unfold intersect
-      simp
-      split
-      . rename_i h
-        rw [← Classifier.subclass_is_Subclass] at h
-        apply! singleton_l
-      . split
-        . rename_i h
-          rw [← Classifier.subclass_is_Subclass] at h
-          apply! singleton_r
-        . rename_i h1 h2
-          rw [← Classifier.subclass_is_Subclass] at h1 h2
-          cases Classifier.subclass_or_disjoint r1 r2 <;> try contradiction
-          rename_i h3; cases h3
-          case inl h3 => have h4 := h3.weaken; contradiction
-          case inr h3 => apply! singleton_disj
-
-theorem Kind.Intersect.top_r {K : Kind} : K.intersect .top = K := by
-  induction K
-  case empty => simp
-  case union ha hb => simp_all
-  case node r1 ex1 =>
-    have h := Classifier.Subclass.of_top (a:=r1)
-    rw [Classifier.subclass_is_Subclass] at h
-    aesop
-
-theorem Kind.Intersect.top_l {K : Kind} : Kind.top.intersect K = K := by
-  induction K
-  case empty => simp
-  case union ha hb => aesop
-  case node r1 ex1 =>
-    have h := Classifier.Subclass.of_top (a:=r1)
-    rw [Classifier.subclass_is_Subclass] at h
-    simp
-    split
-    . rename_i h1; unfold Classifier.subclass at h1; simp_all
-    . simp
-
-theorem Kind.Intersect.assoc {A B C : Kind} : (A.intersect B).intersect C = A.intersect (B.intersect C) := by
-  -- will be correct when we flatten the structure
-  sorry
-
-inductive Kind.Subtract : Kind -> Kind -> Kind -> Prop where
-  | empty_l : Subtract .empty K .empty
-  | union_l : Subtract K1 K R1 -> Subtract K2 K R2 -> Subtract (.union K1 K2) K (.union R1 R2)
-  | empty_r : Subtract (.node r1 ex1) .empty (.node r1 ex1)
-  | union_r :
-    Subtract (.node r1 ex1) K1 R1 ->
-    Subtract R1 K2 R2 ->
-    Subtract (.node r1 ex1) (.union K1 K2) R2
-  -- The singleton cases
-  -- Basically we follow a few broad strokes:
-  -- - A \ (B \ C) = (A \ B) ∪ (A ∩ B ∩ C)
-  -- - For B of the form (.node r []) (no exclusion):
-  --   - If r < A, refine A
-  --   - If r > A, empty
-  --   - If r ⊥ A, A
-  -- Base case first
-  | tree : Subtract (.node r1 ex1) (.node r2 []) (.node r1 (r2 :: ex1))
-  -- Exclusion case
-  -- First, handle the cases where (B \ C) doesn't make sense
-  | excl_absurd_r :
-    r2.StrictSub a -> -- (B \ a) is just empty
-    Subtract (.node r1 ex1) (.node r2 (a :: ex2)) (.node r1 ex1)
-  | excl_irrelevant_r :
-    r2.Disjoint a -> -- (B \ a) = B
-    Subtract (.node r1 ex1) (.node r2 ex2) R ->
-    Subtract (.node r1 ex1) (.node r2 (a :: ex2)) R
-  -- Now, for cases where a is a subtree of r2
-  -- We use the formula A \ (B \ C) = (A \ B) ∪ (A ∩ B ∩ C)
-  | excl_subclass_r :
-    a.Subclass r2 ->
-    a.Subclass r1 -> -- A ∩ B ∩ C = a with all the exclusions
-    Subtract (.node r1 ex1) (.node r2 ex2) R ->
-    Subtract (.node r1 ex1) (.node r2 (a :: ex2)) (.union R (.node a ex1))
-                                        -- ^ we'd need (ex1 ++ ex2) here to be exact,
-                                        -- but if an element is in the ex2 subtree
-                                        -- and not already excluded from A, it is part
-                                        -- of (A \ B), so it's okay to keep anyway.
-  | excl_subclass_l :
-    a.Subclass r2 ->
-    r1.StrictSub a ->  -- B \ C excludes the entirety of A
-    Subtract (.node r1 ex1) (.node r2 (a :: ex2)) (.node r1 ex1)
-  | excl_irrelevant_l :
-    a.Subclass r2 ->
-    r1.Disjoint a -> -- irrelevant exclusion, A ∪ B ∪ C = empty
-    Subtract (.node r1 ex1) (.node r2 ex2) R ->
-    Subtract (.node r1 ex1) (.node r2 (a :: ex2)) R
-
-inductive Kind.Subkind : Kind -> Kind -> Prop where
-  | subtract : Subtract K1 K2 R -> IsEmpty R -> Subkind K1 K2
-
-theorem Kind.Subtract.is_empty_l (hs : Subtract K1 K2 R) (he : IsEmpty K1) : IsEmpty R := by
-  induction hs
-  case empty_l => constructor
-  case union_l ha hb =>
-    cases he
-    apply! IsEmpty.union (ha _) (hb _)
-  case empty_r => assumption
-  case union_r ha hb =>
-    apply hb
-    apply! ha
-  case tree => constructor; exact .there he.is_absurd
-  case excl_absurd_r => assumption
-  case excl_irrelevant_r ih => apply! ih
-  case excl_subclass_r hs2 hs1 _ ih =>
-    constructor; apply! ih;
-    constructor; cases he
-    apply! ContainsSupOf.trans_subclass
-  case excl_subclass_l hs2 hs1 => assumption
-  case excl_irrelevant_l ih => apply! ih
-
-
-theorem Kind.Subtract.absurd_l (hs : Subtract (.node r1 ex1) K R) (hsc : ContainsSupOf ex1 r1) : IsEmpty R := by
-  apply hs.is_empty_l
-  constructor
-  assumption
-
-theorem Kind.Subtract.empty_implies_subclass
-  (hs : Subtract (.node r1 ex1) (.node r2 ex2) R)
-  (he : IsEmpty R)
-  : ContainsSupOf ex1 r1 ∨ r1.Subclass r2 := by
-  cases hs
-  case tree =>
-    cases he.is_absurd <;> aesop
-  case excl_absurd_r => left; apply he.is_absurd
-  case excl_irrelevant_r hs => apply hs.empty_implies_subclass he
-  case excl_subclass_r hs =>
-    cases he
-    apply! hs.empty_implies_subclass
-  case excl_subclass_l => left; apply he.is_absurd
-  case excl_irrelevant_l hs => apply! hs.empty_implies_subclass
-
-theorem Kind.Subtract.empty_r_inv (hs : Subtract K1 K2 R) (he : IsEmpty R) (hek2 : IsEmpty K2) : IsEmpty K1 := by
-  induction hs
-  case empty_l => constructor
-  case union_l ha hb =>
-    cases he
-    constructor
-    apply! ha
-    apply! hb
-  case empty_r => assumption
-  case union_r ha hb =>
-    cases hek2
-    simp_all
-  case tree => cases hek2.is_absurd
-  case excl_absurd_r hs => assumption
-  case excl_irrelevant_r hd hs ih =>
-    cases hek2.is_absurd
-    case here hsk => cases hd.not_subclass hsk
-    case there hek2 => apply! ih _ (.absurd hek2)
-  case excl_subclass_r hs2 hs1 hs ih =>
-    cases he
-    cases hek2.is_absurd
-    case here hsk =>
-      cases hs2.antisymm hsk
-      rename_i h _
-      cases hs.empty_implies_subclass h
-      case inl => constructor; assumption
-      case inr hsk2 => cases hsk2.antisymm hs1; assumption
-    case there hsk => apply! ih _ (.absurd _)
-  case excl_subclass_l => assumption
-  case excl_irrelevant_l hs2 hd1 hs ih =>
-    cases hek2.is_absurd
-    case here hsa =>
-      cases hs2.antisymm hsa
-      cases hs.empty_implies_subclass he
-      case inl h1 => exact .absurd h1
-      case inr h1 => cases hd1.not_subclass h1
-    case there hsc => apply ih he (.absurd hsc)
-
-theorem Kind.Subkind.empty_r_inv (hs : Subkind K1 K2) (he : IsEmpty K2) : IsEmpty K1 := by
-  cases hs
-  apply! Subtract.empty_r_inv
-
-inductive Kind.Disjoint : Kind -> Kind -> Prop where
-  | empty_l: Disjoint .empty K
-  | empty_r : Disjoint K .empty
-  | union_l : Disjoint K1 K -> Disjoint K2 K -> Disjoint (K1.union K2) K
-  | union_r : Disjoint K K1 -> Disjoint K K2 -> Disjoint K (K1.union K2)
-  | absurd_l : ContainsSupOf ex1 r1 -> Disjoint (.node r1 ex1) (.node r2 ex2)
-  | absurd_r : ContainsSupOf ex2 r2 -> Disjoint (.node r1 ex1) (.node r2 ex2)
-  | root : r1.Disjoint r2 -> Disjoint (.node r1 ex1) (.node r2 ex2)
-  | excl_l : ContainsSupOf ex2 r1 -> Disjoint (.node r1 ex1) (.node r2 ex2)
-  | excl_r : ContainsSupOf ex1 r2 -> Disjoint (.node r1 ex1) (.node r2 ex2)
-
-theorem Kind.Disjoint.union_l_inv (hd : Disjoint (K1.union K2) K) : Disjoint K1 K ∧ Disjoint K2 K := by
-  generalize hk : Kind.union K1 K2 = K' at hd
-  induction hd with
-  | empty_l => cases hk
-  | empty_r => exact ⟨.empty_r, .empty_r⟩
-  | union_l hd1 hd2 =>
-    cases hk
-    exact ⟨hd1, hd2⟩
-  | union_r hd1 hd2 ih1 ih2 =>
-    have ⟨hd1', hd2'⟩ := ih1 hk
-    have ⟨hd1'', hd2''⟩ := ih2 hk
-    exact ⟨.union_r hd1' hd1'', .union_r hd2' hd2''⟩
-  | absurd_l => cases hk
-  | absurd_r => cases hk
-  | root => cases hk
-  | excl_l => cases hk
-  | excl_r => cases hk
-
-theorem Kind.Disjoint.union_r_inv (hd : Disjoint K (K1.union K2)) : Disjoint K K1 ∧ Disjoint K K2 := by
-  generalize hk : Kind.union K1 K2 = K' at hd
-  induction hd with
-  | empty_l => exact ⟨.empty_l, .empty_l⟩
-  | empty_r => cases hk
-  | union_l hd1 hd2 ih1 ih2 =>
-    have ⟨hd1', hd2'⟩ := ih1 hk
-    have ⟨hd1'', hd2''⟩ := ih2 hk
-    exact ⟨.union_l hd1' hd1'', .union_l hd2' hd2''⟩
-  | union_r hd1 hd2 =>
-    cases hk
-    exact ⟨hd1, hd2⟩
-  | absurd_l => cases hk
-  | absurd_r => cases hk
-  | root => cases hk
-  | excl_l => cases hk
-  | excl_r => cases hk
-
-theorem Kind.Disjoint.implies_empty_intersect (hd : K1.Disjoint K2) (hi : Intersect K1 K2 R) : IsEmpty R := by
-  induction hi with
-  | empty_l => exact .empty
-  | empty_r => exact .empty
-  | union_l hi1 hi2 ih1 ih2 =>
-    have ⟨hd1, hd2⟩ := hd.union_l_inv
-    exact .union (ih1 hd1) (ih2 hd2)
-  | union_r hi1 hi2 ih1 ih2 =>
-    have ⟨hd1, hd2⟩ := hd.union_r_inv
-    exact .union (ih1 hd1) (ih2 hd2)
-  | singleton_l hs =>
-    cases hd with
-    | absurd_l ha => exact .absurd (.append_l ha)
-    | absurd_r ha => exact .absurd (.append_r (ha.trans_subclass hs))
-    | root hd => cases hd.not_subclass hs
-    | excl_l ha => exact .absurd (.append_r ha)
-    | excl_r ha => exact .absurd (.append_l (ha.trans_subclass hs))
-  | singleton_r hs =>
-    cases hd with
-    | absurd_l ha => exact .absurd (.append_l (ha.trans_subclass hs))
-    | absurd_r ha => exact .absurd (.append_r ha)
-    | root hd => cases hd.symm.not_subclass hs
-    | excl_l ha => exact .absurd (.append_r (ha.trans_subclass hs))
-    | excl_r ha => exact .absurd (.append_l ha)
-  | singleton_disj => exact .empty
-
-theorem Kind.Disjoint.from_empty_intersect (hi : Intersect K1 K2 R) (he : IsEmpty R) : K1.Disjoint K2 := by
-  induction hi with
-  | empty_l => exact .empty_l
-  | empty_r => exact .empty_r
-  | union_l hi1 hi2 ih1 ih2 =>
-    cases he with
-    | union he1 he2 => exact .union_l (ih1 he1) (ih2 he2)
-  | union_r hi1 hi2 ih1 ih2 =>
-    cases he with
-    | union he1 he2 => exact .union_r (ih1 he1) (ih2 he2)
-  | singleton_l hs =>
-    cases he with
-    | absurd ha =>
-      cases ha.of_append with
-      | inl ha => exact .absurd_l ha
-      | inr ha => exact .excl_l ha
-  | singleton_r hs =>
-    cases he with
-    | absurd ha =>
-      cases ha.of_append with
-      | inl ha => exact .excl_r ha
-      | inr ha => exact .absurd_r ha
-  | singleton_disj hd => exact .root hd
-
-theorem Kind.Disjoint.top_l (hd: Disjoint .top K) : IsEmpty K := by
-  cases hd
-  case empty_r => constructor
-  case union_r ha hb => apply IsEmpty.union ha.top_l hb.top_l
-  case absurd_l hsc => cases hsc
-  case absurd_r hsc => constructor; assumption
-  case root hd => cases hd.symm.not_subclass .of_top
-  case excl_l hsc => constructor; apply hsc.trans_subclass .of_top
-  case excl_r hsc => cases hsc
-
-theorem Kind.Disjoint.symm (hd : K1.Disjoint K2) : Disjoint K2 K1 := by
-  induction hd with
-  | empty_l => exact .empty_r
-  | empty_r => exact .empty_l
-  | union_l _ _ ih1 ih2 => exact .union_r ih1 ih2
-  | union_r _ _ ih1 ih2 => exact .union_l ih1 ih2
-  | absurd_l ha => exact .absurd_r ha
-  | absurd_r ha => exact .absurd_l ha
-  | root hd => exact .root hd.symm
-  | excl_l ha => exact .excl_r ha
-  | excl_r ha => exact .excl_l ha
-
-theorem Kind.Disjoint.append_excl_l (hd : Disjoint (.node r1 ex2) K) : Disjoint (.node r1 (ex1 ++ ex2)) K := by
-  cases hd
-  case empty_r => apply! empty_r
-  case union_r ha hb => apply union_r ha.append_excl_l hb.append_excl_l
-  case absurd_l ha => apply absurd_l ha.append_r
-  case absurd_r => apply! absurd_r
-  case root => apply! root
-  case excl_l => apply! excl_l
-  case excl_r ha => apply excl_r ha.append_r
-
-theorem Kind.Disjoint.refine_subroot_l (hd : Disjoint (.node r1 ex1) K) (hs : r2.Subclass r1) : Disjoint (.node r2 ex1) K := by
-  cases hd
-  case empty_r => apply! empty_r
-  case union_r ha hb => apply! union_r (ha.refine_subroot_l _) (hb.refine_subroot_l _)
-  case absurd_l ha => apply! absurd_l $ ha.trans_subclass _
-  case absurd_r => apply! absurd_r
-  case root hdr => apply root; apply! hdr.refines_subclass_l _
-  case excl_l hc => apply! excl_l $ hc.trans_subclass _
-  case excl_r => apply! excl_r
-
--- If K1 is disjoint from K', and R is the intersection of K with K1, then R is disjoint from K'
-theorem Kind.Disjoint.intersect_disjoint (hd : K1.Disjoint K') (hi : Intersect K K1 R) : R.Disjoint K' := by
-  induction hi
-  case empty_l => apply! empty_l
-  case empty_r => apply! empty_l
-  case union_l iha ihb => apply! union_l (iha _) (ihb _)
-  case union_r iha ihb =>
-    have ⟨_, _⟩ := hd.union_l_inv
-    apply! union_l (iha _) (ihb _)
-  case singleton_l hs => apply append_excl_l; apply! hd.refine_subroot_l _
-  case singleton_r hs => apply hd.append_excl_l
-  case singleton_disj hdr => apply empty_l
-
-theorem Kind.Disjoint.absurd_l' (hs : ContainsSupOf ex1 r1) : Disjoint (.node r1 ex1) K := by
-  induction K
-  case empty => apply empty_r
-  case node => apply! absurd_l
-  case union ha hb => apply! union_r
-
-theorem Kind.Disjoint.refine_subtract_l (hd : Disjoint K1 K) (hs : Subtract K1 K2 R) : Disjoint R K := by
-  induction hs
-  case empty_l => exact .empty_l
-  case union_l ih1 ih2 =>
-    have ⟨hd1, hd2⟩ := hd.union_l_inv
-    exact .union_l (ih1 hd1) (ih2 hd2)
-  case empty_r => assumption
-  case union_r ih1 ih2 => exact ih2 (ih1 hd)
-  case tree => apply! hd.append_excl_l (ex1 := [_])
-  case excl_absurd_r => assumption
-  case excl_irrelevant_r ih => apply! ih
-  case excl_subclass_r hs1 _ ih =>
-    apply Disjoint.union_l
-    apply! ih
-    apply! hd.refine_subroot_l
-  case excl_subclass_l => assumption
-  case excl_irrelevant_l ih => apply! ih
-
-theorem Kind.Disjoint.append_l_disj_inv (hd : Disjoint (.node r1 (a :: ex1)) (.node r2 ex2)) (hda : a.Disjoint r2) : Disjoint (.node r1 ex1) (.node r2 ex2) := by
-  cases hd
-  case absurd_l hsc =>
-    cases hsc
-    case here hs => apply! root $ hda.refines_subclass_l _
-    case there hsc => apply! absurd_l
-  case absurd_r => apply! absurd_r
-  case root => apply! root
-  case excl_l hsc => apply! excl_l
-  case excl_r hsc =>
-    cases hsc
-    case here hs => cases hda.symm.not_subclass hs
-    case there => apply! excl_r
-
-theorem Kind.Disjoint.append_l_contained_inv (hd : Disjoint (.node r1 (a :: ex1)) (.node r2 ex2)) (hsc: ContainsSupOf ex2 a) : Disjoint (.node r1 ex1) (.node r2 ex2) := by
-  cases hd
-  case absurd_l hsc =>
-    cases hsc
-    case here hs => apply! excl_l $ hsc.trans_subclass _
-    case there hsc => apply! absurd_l
-  case absurd_r => apply! absurd_r
-  case root => apply! root
-  case excl_l hsc => apply! excl_l
-  case excl_r hsc =>
-    cases hsc
-    case here hs => apply! absurd_r $ hsc.trans_subclass _
-    case there => apply! excl_r
-
-theorem Kind.Disjoint.refine_disjoint_subtract_l_disjoint_root
-  (hdr : Disjoint R K)
-  (hs : Subtract (.node r1 ex1) (.node r2 ex2) R)
-  (hd : r1.Disjoint r2)
-  : Disjoint (.node r1 ex1) K := by
-  cases hs
-  case tree =>
-    generalize h : node r1 (r2 :: ex1) = L at hdr
-    induction hdr <;> try cases h
-    case empty_r => apply! empty_r
-    case union_r ha hb => simp_all; apply! union_r
-    case absurd_l hsc =>
-      cases hsc
-      case here hs => cases hd.not_subclass hs
-      case there hsc => apply! absurd_l
-    case absurd_r => apply! absurd_r
-    case root hd2 => apply! root
-    case excl_l => apply! excl_l
-    case excl_r hsc =>
-      cases hsc
-      case here hs => apply! root $ hd.refines_subclass_r _
-      case there hsc => apply! excl_r
-  case excl_absurd_r => assumption
-  case excl_irrelevant_r hs => apply! hdr.refine_disjoint_subtract_l_disjoint_root
-  case excl_subclass_r hs =>
-    have ⟨hl, _⟩ := hdr.union_l_inv
-    apply! hl.refine_disjoint_subtract_l_disjoint_root _ hd
-  case excl_subclass_l => assumption
-  case excl_irrelevant_l hs => apply! hdr.refine_disjoint_subtract_l_disjoint_root
-
-theorem Kind.Disjoint.refine_disjoint_subtract_l_subroot
-  (hdr : Disjoint R K)
-  (hs : Subtract (.node r1 ex1) (.node r2 ex2) R)
-  (hsub : r2.Subclass r1)
-  (hd2 : Disjoint (.node r2 ex1) K)
-  : Disjoint (.node r1 ex1) K := by
-  cases hs
-  case tree =>
-    generalize h : node r1 (r2 :: ex1) = L at hdr
-    induction hdr <;> try cases h
-    case empty_r => apply! empty_r
-    case union_r ha hb =>
-      have ⟨_, _⟩ := hd2.union_r_inv
-      simp_all
-      apply! union_r
-    case absurd_l hsc =>
-      cases hsc
-      case here hs2 => cases hsub.antisymm hs2; assumption
-      case there => apply! absurd_l
-    case absurd_r => apply! absurd_r
-    case root => apply! root
-    case excl_l => apply! excl_l
-    case excl_r hsc =>
-      cases hsc
-      case here hs2 =>
-        cases hd2
-        case absurd_l => apply excl_r; apply! ContainsSupOf.trans_subclass
-        case absurd_r => apply! absurd_r
-        case root hd => cases hd.symm.not_subclass hs2
-        case excl_l hsc => apply! absurd_r $ hsc.trans_subclass _
-        case excl_r hsc => apply! excl_r
-      case there hsc => apply! excl_r
-  case excl_absurd_r => assumption
-  case excl_irrelevant_r hs =>  apply! hdr.refine_disjoint_subtract_l_subroot
-  case excl_subclass_r hs =>
-    have ⟨hl, _⟩ := hdr.union_l_inv
-    apply! hl.refine_disjoint_subtract_l_subroot
-  case excl_subclass_l => assumption
-  case excl_irrelevant_l hs => apply! hdr.refine_disjoint_subtract_l_subroot
-
-
-
-theorem Kind.Disjoint.refine_disjoint_subtract_l (hd2 : Disjoint K2 K) (hs : Subtract K1 K2 R) (hdr : Disjoint R K) : Disjoint K1 K := by
-  induction hs generalizing K
-  case empty_l => apply empty_l
-  case union_l ih1 ih2 =>
-    have ⟨_, _⟩ := hdr.union_l_inv
-    apply! union_l (ih1 _ _) (ih2 _ _)
-  case empty_r => assumption
-  case union_r ha hb =>
-    have ⟨hl, hr⟩ := hd2.union_l_inv
-    apply ha hl _
-    apply hb hr hdr
-  case tree r1 ex1 r2 =>
-    generalize h : node r1 (r2 :: ex1) = L at hdr
-    induction hdr <;> try cases h
-    case empty_r => apply! empty_r
-    case union_r ha hb =>
-      have ⟨_, _⟩ := hd2.union_r_inv
-      simp_all
-      apply! union_r
-    case absurd_l hsc =>
-      cases hsc
-      case here hs =>
-        cases hd2
-        case absurd_l hsc => cases hsc
-        case absurd_r hsc => apply! absurd_r
-        case root hd =>  apply root; apply! hd.refines_subclass_l _
-        case excl_l hsc => apply excl_l; apply! hsc.trans_subclass
-        case excl_r hsc => cases hsc
-      case there hsc => apply! absurd_l
-    case absurd_r => apply! absurd_r
-    case root => apply! root
-    case excl_l => apply! excl_l
-    case excl_r hsc =>
-      cases hsc
-      case here hs =>
-        cases hd2
-        case absurd_r hsc => apply! absurd_r
-        case root hd => cases hd.symm.not_subclass hs
-        case excl_l hsc => apply absurd_r; apply! hsc.trans_subclass
-        case excl_r hsc => cases hsc
-        case absurd_l hsc => cases hsc
-      case there hsc => apply! excl_r
-  case excl_subclass_r r1 ex1 r2 ex2 _ a hss hsc hs ih =>
-    have ⟨hdr1, hdr2⟩ := hdr.union_l_inv
-    generalize h : node r2 (a :: ex2) = L at hd2
-    induction hd2 generalizing K2 <;> try cases h
-    case empty_r => apply! empty_r
-    case union_r ha hb =>
-      simp_all
-      have ⟨_, _⟩ := hdr.union_r_inv
-      have ⟨_, _⟩ := hdr1.union_r_inv
-      have ⟨_, _⟩ := hdr2.union_r_inv
-      apply! union_r (ha _ _ _) (hb _ _ _)
-    case absurd_l hsc =>
-      cases hsc
-      case here hsc1 =>
-        cases hss.antisymm hsc1
-        apply! hdr1.refine_disjoint_subtract_l_subroot
-      case there hsc =>
-        apply ih _ hdr1
-        apply! absurd_l
-    case absurd_r => apply! absurd_r
-    case root hd1 => apply ih (.root hd1) hdr1
-    case excl_l hsc => apply! ih (.excl_l _)
-    case excl_r hsc =>
-      cases hsc
-      case here hs =>
-        cases hdr2
-        case absurd_l hsc => apply! excl_r $ hsc.trans_subclass _
-        case absurd_r => apply! absurd_r
-        case root hd => cases hd.symm.not_subclass hs
-        case excl_l hsc => apply! absurd_r $ hsc.trans_subclass _
-        case excl_r => apply! excl_r
-      case there hsc => apply! ih (excl_r _)
-  case excl_absurd_r hs => assumption
-  case excl_irrelevant_r r1 ex1 r2 ex2 _ a hd hs ih =>
-    generalize h : node r2 (a :: ex2) = L at hd2
-    induction hd2 generalizing K2 <;> try cases h
-    case empty_r => apply! empty_r
-    case union_r ha hb =>
-      simp_all
-      have ⟨_, _⟩ := hdr.union_r_inv
-      apply! union_r (ha _) (hb _)
-    case absurd_l hsc =>
-      cases hsc
-      case here hsc => cases hd.not_subclass hsc
-      case there hsc =>
-        apply ih _ hdr
-        apply! absurd_l
-    case absurd_r => apply! absurd_r
-    case root hd1 => apply ih (.root hd1) hdr
-    case excl_l hsc => apply! ih (.excl_l _)
-    case excl_r hsc =>
-      cases hsc
-      case here hs => apply ih _ hdr; apply root; apply! hd.refines_subclass_r
-      case there hsc => apply! ih (excl_r _)
-  case excl_subclass_l hs2 hs1 => assumption
-  case excl_irrelevant_l r1 ex1 r2 ex2 _ a hs2 hd1 hs ih =>
-    generalize h : node r2 (a :: ex2) = L at hd2
-    induction hd2 generalizing K2 <;> try cases h
-    case empty_r => apply! empty_r
-    case union_r ha hb =>
-      simp_all
-      have ⟨_, _⟩ := hdr.union_r_inv
-      apply! union_r (ha _) (hb _)
-    case absurd_l hsc =>
-      cases hsc
-      case here hsc =>
-        cases hs2.antisymm hsc
-        apply! hdr.refine_disjoint_subtract_l_disjoint_root hs
-      case there hsc =>
-        apply ih _ hdr
-        apply! absurd_l
-    case absurd_r => apply! absurd_r
-    case root hd1 => apply ih (.root hd1) hdr
-    case excl_l hsc => apply! ih (.excl_l _)
-    case excl_r hsc =>
-      cases hsc
-      case here hs => apply root; apply! hd1.refines_subclass_r
-      case there hsc => apply! ih (excl_r _)
-
-theorem Kind.Disjoint.is_empty_l (he : IsEmpty K) : Disjoint K L := by
-  induction he
-  case empty => apply empty_l
-  case absurd => apply! absurd_l'
-  case union ha hb => apply! union_l
-
-theorem Kind.Disjoint.refine_subkind_l' (hd : Disjoint K2 K) (hs : Subtract K1 K2 R) (he : IsEmpty R) : Disjoint K1 K := by
-  apply refine_disjoint_subtract_l hd hs
-  apply is_empty_l he
-
-theorem Kind.Disjoint.refine_subkind_l (hd : Disjoint K2 K) (hs : Subkind K1 K2) : Disjoint K1 K := by
-  cases hs
-  apply! hd.refine_subkind_l'
-
-theorem Kind.Subkind.refine_disjoint_l (hs : Subkind K1 K2) (hd : Disjoint K2 K) : Disjoint K1 K := hd.refine_subkind_l hs
-
-theorem Kind.Subtract.exists' : ∃ R, Subtract (node r1 ex1) (node r2 ex2) R := by
-  induction ex2
-  case nil => exists node r1 (r2 :: ex1); apply tree
-  case cons head tail ih =>
-    cases head.subclass_or_disjoint r2
-    case inl hs =>
-      have ⟨R, h⟩ := ih
-      cases head.subclass_or_disjoint r1
-      case inl hs1 =>
-        exists .union R (.node head ex1)
-        apply! excl_subclass_r
-      case inr hs1 =>
-        cases hs1
-        case inl hs1 =>
-          exists node r1 ex1
-          apply! excl_subclass_l
-        case inr hs1 =>
-          exists R
-          apply! excl_irrelevant_l _ hs1.symm
-    case inr hs =>
-      cases hs
-      case inl hs =>
-        exists node r1 ex1
-        apply! excl_absurd_r
-      case inr hs =>
-        have ⟨R, h⟩ := ih
-        exists R
-        apply! excl_irrelevant_r hs.symm
-
-theorem Kind.Subtract.exists (a : Kind) (b: Kind) : ∃ R, Subtract a b R := by
-  induction b generalizing a
-  case empty =>
-    induction a
-    case empty => exists empty; apply! empty_l
-    case node r1 ex1 => exists node r1 ex1; apply empty_r
-    case union ha hb =>
-      have ⟨r1, h1⟩ := ha
-      have ⟨r2, h2⟩ := hb
-      exists .union r1 r2
-      apply! union_l
-  case union hb1 hb2 =>
-    induction a
-    case empty => exists empty; apply! empty_l
-    case node r1 ex1 =>
-      have ⟨r1, h1⟩ := hb1 (a := node r1 ex1)
-      have ⟨r2, h2⟩ := hb2 (a := r1)
-      exists r2; apply! union_r
-    case union ha1 ha2 =>
-      have ⟨r1, h1⟩ := ha1
-      have ⟨r2, h2⟩ := ha2
-      exists .union r1 r2
-      apply! union_l
-  case node r2 ex2 =>
-    induction a
-    case empty => exists empty; apply! empty_l
-    case node r1 ex1 =>
-      apply exists'
-    case union ha1 ha2 =>
-      have ⟨r1, h1⟩ := ha1
-      have ⟨r2, h2⟩ := ha2
-      exists .union r1 r2
-      apply! union_l
 
 theorem Kind.Subtract.is_empty_append_l
   (hs : Subtract (.node r1 ex1) (.node r2 ex2) R)
@@ -1383,62 +756,62 @@ theorem Kind.ContainsSupOf.lawful : ContainsSupOf exs r ↔ contains_sup_of exs 
       . apply ContainsSupOf.here; simp_all [Classifier.subclass_is_Subclass]
       . apply ContainsSupOf.there; rw [← lawful] at hsc; simp_all
 
-@[simp]
-def Kind.disjoint (K1 : Kind) (K2 : Kind) :=
-  match K1 with
-  | .empty => true
-  | .union a b => a.disjoint K2 && b.disjoint K2
-  | .node r1 ex1 =>
-    match K2 with
-    | .empty => true
-    | .union a b => (Kind.node r1 ex1).disjoint a && (Kind.node r1 ex1).disjoint b
-    | .node r2 ex2 =>
-      r1.disjoint r2
-        || contains_sup_of ex1 r1 || contains_sup_of ex2 r2
-        || contains_sup_of ex1 r2 || contains_sup_of ex2 r1
+-- @[simp]
+-- def Kind.disjoint (K1 : Kind) (K2 : Kind) :=
+--   match K1 with
+--   | .empty => true
+--   | .union a b => a.disjoint K2 && b.disjoint K2
+--   | .node r1 ex1 =>
+--     match K2 with
+--     | .empty => true
+--     | .union a b => (Kind.node r1 ex1).disjoint a && (Kind.node r1 ex1).disjoint b
+--     | .node r2 ex2 =>
+--       r1.disjoint r2
+--         || contains_sup_of ex1 r1 || contains_sup_of ex2 r2
+--         || contains_sup_of ex1 r2 || contains_sup_of ex2 r1
 
-theorem Kind.Disjoint.lawful : Disjoint K1 K2 ↔ K1.disjoint K2 := by
-  apply Iff.intro
-  . intro hd
-    induction hd
-    case empty_l => simp
-    case empty_r K =>
-      induction K <;> simp_all
-    case union_l => simp_all
-    case union_r K K1 K2 _ _ ha hb =>
-      induction K <;> simp_all
-      rename_i iha ihb hha hhb
-      have ⟨_, _⟩ := hha.union_l_inv
-      have ⟨_, _⟩ := hhb.union_l_inv
-      apply And.intro
-      apply! iha
-      apply! ihb
-    case absurd_l hsc => simp_all [ContainsSupOf.lawful]
-    case absurd_r hsc => simp_all [ContainsSupOf.lawful]
-    case root hd => simp_all [Classifier.disjoint_is_Disjoint]
-    case excl_l => simp_all [ContainsSupOf.lawful]
-    case excl_r => simp_all [ContainsSupOf.lawful]
-  . intro hd
-    induction K1
-    case empty => apply empty_l
-    case union ha hb =>
-      apply union_l <;> simp_all
-    case node r1 ex1 =>
-      induction K2
-      case empty => apply empty_r
-      case union ha hb =>
-        apply union_r <;> simp_all
-      case node r2 ex2 =>
-        simp at hd; rw [← Classifier.disjoint_is_Disjoint] at hd; repeat rw [← ContainsSupOf.lawful] at hd
-        cases hd <;> rename_i hd
-        . cases hd <;> rename_i hd
-          . cases hd <;> rename_i hd
-            . cases hd <;> rename_i hd
-              . apply! root
-              . apply! absurd_l
-            . apply! absurd_r
-          . apply! excl_r
-        . apply! excl_l
+-- theorem Kind.Disjoint.lawful : Disjoint K1 K2 ↔ K1.disjoint K2 := by
+--   apply Iff.intro
+--   . intro hd
+--     induction hd
+--     case empty_l => simp
+--     case empty_r K =>
+--       induction K <;> simp_all
+--     case union_l => simp_all
+--     case union_r K K1 K2 _ _ ha hb =>
+--       induction K <;> simp_all
+--       rename_i iha ihb hha hhb
+--       have ⟨_, _⟩ := hha.union_l_inv
+--       have ⟨_, _⟩ := hhb.union_l_inv
+--       apply And.intro
+--       apply! iha
+--       apply! ihb
+--     case absurd_l hsc => simp_all [ContainsSupOf.lawful]
+--     case absurd_r hsc => simp_all [ContainsSupOf.lawful]
+--     case root hd => simp_all [Classifier.disjoint_is_Disjoint]
+--     case excl_l => simp_all [ContainsSupOf.lawful]
+--     case excl_r => simp_all [ContainsSupOf.lawful]
+--   . intro hd
+--     induction K1
+--     case empty => apply empty_l
+--     case union ha hb =>
+--       apply union_l <;> simp_all
+--     case node r1 ex1 =>
+--       induction K2
+--       case empty => apply empty_r
+--       case union ha hb =>
+--         apply union_r <;> simp_all
+--       case node r2 ex2 =>
+--         simp at hd; rw [← Classifier.disjoint_is_Disjoint] at hd; repeat rw [← ContainsSupOf.lawful] at hd
+--         cases hd <;> rename_i hd
+--         . cases hd <;> rename_i hd
+--           . cases hd <;> rename_i hd
+--             . cases hd <;> rename_i hd
+--               . apply! root
+--               . apply! absurd_l
+--             . apply! absurd_r
+--           . apply! excl_r
+--         . apply! excl_l
 
 
 -- inductive Kind.Contains : Kind -> Classifier -> Prop where
