Capless/Classifier/Intersection.lean
@@ -1,0 +1,173 @@
+import Capless.Classifier.Core
+import Capless.Classifier.Kind
+
+namespace Capless
+
+/-- The intersection of two subtrees. -/
+inductive Subtree.Intersect : Subtree -> Subtree -> Kind -> Prop where
+  | subtree_l : r1.Subclass r2 -> Intersect (mk r1 ex1) (mk r2 ex2) [mk r1 (ex1 ++ ex2)]
+  | subtree_r : r2.Subclass r1 -> Intersect (mk r1 ex1) (mk r2 ex2) [mk r2 (ex1 ++ ex2)]
+  | disjoint : r1.Disjoint r2 -> Intersect (mk r1 ex1) (mk r2 ex2) []
+
+/-- Intersection of two kinds. -/
+inductive Kind.Intersect : Kind -> Kind -> Kind -> Prop where
+  | empty_l : Intersect [] K []
+  | empty_r : Intersect K [] []
+  | append_l : Intersect [x] K R1 -> Intersect xs K R2 -> Intersect (x::xs) K (R1 ++ R2)
+  | append_r : Intersect K [x] R1 -> Intersect K xs R2 -> Intersect K (x::xs) (R1 ++ R2)
+  | singleton : x.Intersect y R -> Intersect [x] [y] R
+
+@[simp]
+def Subtree.intersect (s : Subtree) (t : Subtree) : Kind :=
+  if s.root.subclass t.root then .node s.root (s.excls ++ t.excls)
+  else if t.root.subclass s.root then .node t.root (s.excls ++ t.excls)
+  else .empty
+
+theorem Subtree.Intersect.lawful : Intersect s t (s.intersect t) := by
+  simp
+  split
+  . rename_i h
+    simp [← Classifier.subclass_is_Subclass] at h
+    apply! subtree_l
+  . split
+    . rename_i h
+      simp [← Classifier.subclass_is_Subclass] at h
+      apply! subtree_r
+    . simp [← Classifier.subclass_is_Subclass] at *
+      cases Classifier.subclass_or_disjoint s.root t.root <;> rename_i h
+      . contradiction
+      . cases h <;> rename_i h
+        . have h0 := h.weaken; contradiction
+        . simp [← Classifier.disjoint_is_Disjoint] at h
+          apply! disjoint
+
+@[simp]
+def Kind.intersect (k : Kind) (l : Kind) : Kind :=
+  List.flatMap (fun x => List.flatMap (fun y => x.intersect y) l) k
+
+def Kind.intersect.cons_l : intersect (x :: xs) K = intersect [x] K ++ intersect xs K := by simp
+def Kind.intersect.append_l : intersect (xs1 ++ xs2) K = intersect xs1 K ++ intersect xs2 K := by simp
+def Kind.intersect.cons_r : intersect [x] (y :: ys) = intersect [x] [y] ++ intersect [x] ys := by simp
+def Kind.intersect.append_r : intersect [x] (ys1 ++ ys2) = intersect [x] ys1 ++ intersect [x] ys2 := by simp
+
+theorem Kind.Intersect.lawful' : Intersect [x] L (.intersect [x] L) := by
+  induction L
+  case nil => simp; apply empty_r
+  case cons y ys ih =>
+    simp
+    apply append_r
+    . apply singleton .lawful
+    . simp at ih; apply ih
+
+theorem Kind.Intersect.lawful : Intersect K L (K.intersect L) := by
+  induction K generalizing L
+  case nil => simp; apply empty_l
+  case cons x xs ih =>
+    apply append_l _ ih
+    have h := lawful' (x:=x) (L:=L)
+    simp_all
+
+theorem Kind.intersect.top_r {K : Kind} : K.intersect .top = K := by
+  induction K
+  case nil => simp
+  case cons x xs ih =>
+    have h := Classifier.Subclass.of_top (a:=x.root)
+    rw [Classifier.subclass_is_Subclass] at h
+    rw [cons_l, ih]
+    simp [h]
+
+theorem Kind.intersect.top_l {K : Kind} : Kind.top.intersect K = K := by
+  induction K
+  case nil => simp
+  case cons y ys ih =>
+    simp at *
+    rw [ih]
+    cases y
+    rename_i r exs
+    cases r
+    case top => simp [Classifier.subclass]
+    case child n t =>
+      simp [Classifier.subclass]
+      have h := Classifier.Subclass.of_top (a:=t)
+      rw [Classifier.subclass_is_Subclass] at h
+      simp [h]
+
+theorem Classifier.disjoint.implies_no_subclass (hd : disjoint a b) : (a.subclass b = false ∧ b.subclass a = false) := by
+  simp [← Classifier.disjoint_is_Disjoint] at hd
+  simp [← Bool.not_eq_true, ← Classifier.subclass_is_Subclass]
+  apply And.intro
+  . intro h; apply hd.not_subclass h
+  . intro h; apply hd.symm.not_subclass h
+
+theorem Classifier.StrictSub.not_superclass (hss : StrictSub a b) : (b.subclass a = false) := by
+  simp [← Bool.not_eq_true, ← Classifier.subclass_is_Subclass]
+  intro h
+  apply hss.antisymm h
+
+theorem Kind.intersect.assoc'' : (intersect [x] [y]).intersect [z] = intersect [x] (intersect [y] [z]) := by
+  cases Classifier.subclass_or_disjoint x.root y.root <;> rename_i h1
+  . have h1' := Classifier.subclass_is_Subclass.mp h1
+    cases Classifier.subclass_or_disjoint y.root z.root <;> rename_i h2
+    . have h2' := Classifier.subclass_is_Subclass.mp h2
+      have h3' := Classifier.subclass_is_Subclass.mp (h1.trans h2)
+      simp_all
+    . cases h2 <;> rename_i h2
+      . have h2' := Classifier.subclass_is_Subclass.mp h2.weaken
+        have h2'' := h2.not_superclass
+        cases Classifier.subclass_or_disjoint' x.root z.root <;> rename_i h3' <;> aesop
+      . have h2' := Classifier.disjoint_is_Disjoint.mp $ h2.refines_subclass_l h1
+        have ⟨_, _⟩ := Classifier.disjoint.implies_no_subclass h2'
+        have ⟨_, _⟩ := Classifier.disjoint.implies_no_subclass $ Classifier.disjoint_is_Disjoint.mp h2
+        simp_all
+  . cases h1 <;> rename_i h1
+    . have h1' := Classifier.subclass_is_Subclass.mp h1.weaken
+      have h1'' := h1.not_superclass
+      cases Classifier.subclass_or_disjoint y.root z.root <;> rename_i h2
+      . have h2' := Classifier.subclass_is_Subclass.mp h2
+        simp_all
+      . cases h2 <;> rename_i h2
+        . have h2' := Classifier.subclass_is_Subclass.mp h2.weaken
+          have h2'' := h2.not_superclass
+          have h3 := h2.subclass_r h1.weaken
+          have h3' := Classifier.subclass_is_Subclass.mp h3.weaken
+          have h3'' := h3.not_superclass
+          simp_all
+        . have ⟨_, _⟩ := Classifier.disjoint.implies_no_subclass $ Classifier.disjoint_is_Disjoint.mp h2
+          simp_all
+    . have ⟨_, _⟩ := Classifier.disjoint.implies_no_subclass $ Classifier.disjoint_is_Disjoint.mp h1
+      cases Classifier.subclass_or_disjoint y.root z.root <;> rename_i h2
+      . have h2' := Classifier.subclass_is_Subclass.mp h2
+        simp_all
+      . cases h2 <;> rename_i h2
+        . have h2' := Classifier.subclass_is_Subclass.mp h2.weaken
+          have h2'' := h2.not_superclass
+          have h3 := h1.refines_subclass_r h2.weaken
+          have ⟨_, _⟩ := Classifier.disjoint.implies_no_subclass $ Classifier.disjoint_is_Disjoint.mp h3
+          simp_all
+        . have ⟨_, _⟩ := Classifier.disjoint.implies_no_subclass $ Classifier.disjoint_is_Disjoint.mp h2
+          simp_all
+
+theorem Kind.intersect.assoc' {B C : Kind} : (intersect [x] B).intersect C = intersect [x] (B.intersect C) := by
+  induction B generalizing C
+  case nil => simp
+  case cons y ys ih =>
+    rw [cons_l (x:=y), cons_r, append_r, append_l, ih, List.append_left_inj]
+    induction C
+    case nil => simp
+    case cons z zs ih2 =>
+      have h : (intersect [x] [y]).intersect (z :: zs) = (intersect [x] [y]).intersect [z] ++ (intersect [x] [y]).intersect zs := by
+        generalize h0 : intersect [x] [y] = C
+        simp at h0; split at h0
+        . subst_vars; apply cons_r
+        . split at h0;
+          . subst_vars; apply cons_r
+          . subst_vars; simp
+      rw [cons_r (ys:=zs), append_r, h, assoc'', ih2]
+
+theorem Kind.intersect.assoc {A B C : Kind} : (A.intersect B).intersect C = A.intersect (B.intersect C) := by
+  induction A generalizing B C
+  case nil => simp
+  case cons a as ih =>
+    rw [cons_l (xs:=as), cons_l (xs:=as), append_l, ih, List.append_left_inj, assoc']
+
+end Capless
