Capless/Classifier/Kind.lean
@@ -1,0 +1,100 @@
+import Capless.Classifier.Core
+
+namespace Capless
+
+-- **
+-- Kinds
+-- **
+
+/-- A subtree of a single root and an exclusion list.
+    Notionally, it represents the subtree rooted at `root`, excluding the subtrees rooted at `excls`. -/
+structure Subtree : Type where
+  root  : Classifier
+  excls : List Classifier
+
+/-- A classifier filter : a list of filtered subtree. -/
+def Kind : Type := List Subtree
+
+@[simp]
+instance : HAppend Kind Kind Kind where
+  hAppend xs ys := List.append xs ys
+
+/-- A single node. -/
+@[simp]
+def Kind.node (c : Classifier) (excls : List Classifier) : Kind := [Subtree.mk c excls]
+
+/-- Shorthand notation for a subtree without exclusions -/
+@[simp]
+def Kind.classifier (c : Classifier) := Kind.node c []
+
+/-- The empty kind. Note that non-empty kinds can still represent an empty set of nodes. See `IsEmpty`. -/
+@[simp]
+def Kind.empty : Kind := []
+
+/-- The "top" kind. This is a Kind that includes all nodes in the classifier tree. -/
+@[simp]
+def Kind.top := node .top []
+
+/-- Helper relation: does `xs` contain a superclass of `c`? -/
+inductive ContainsSupOf : List Classifier -> Classifier -> Prop where
+  | here : b.Subclass a -> ContainsSupOf (a :: xs) b
+  | there : ContainsSupOf xs b -> ContainsSupOf (a :: xs) b
+
+theorem ContainsSupOf.append_l (h : ContainsSupOf xs b) : ContainsSupOf (xs ++ ys) b := by
+  induction h with
+  | here hs => exact .here hs
+  | there _ ih => exact .there ih
+
+theorem ContainsSupOf.append_r (h : ContainsSupOf ys b) : ContainsSupOf (xs ++ ys) b := by
+  induction xs with
+  | nil => exact h
+  | cons _ _ ih => exact .there ih
+
+theorem ContainsSupOf.trans_subclass (h : ContainsSupOf xs a) (hs : b.Subclass a) : ContainsSupOf xs b := by
+  induction h with
+  | here hs' => exact .here (hs.trans hs')
+  | there _ ih => exact .there (ih hs)
+
+theorem ContainsSupOf.of_append (h : ContainsSupOf (xs ++ ys) b) : ContainsSupOf xs b ∨ ContainsSupOf ys b := by
+  induction xs with
+  | nil => exact .inr h
+  | cons a xs ih =>
+    cases h with
+    | here hs => exact .inl (.here hs)
+    | there h =>
+      cases ih h with
+      | inl h => exact .inl (.there h)
+      | inr h => exact .inr h
+
+/-- Is a Kind empty? -/
+inductive Kind.IsEmpty : Kind -> Prop where
+  | empty : IsEmpty []
+  | absurd : ContainsSupOf exs r -> IsEmpty xs -> IsEmpty (Subtree.mk r exs :: xs)
+
+theorem Kind.IsEmpty.node (hsc : ContainsSupOf exs r) : IsEmpty [.mk r exs] := absurd hsc .empty
+
+/-- If a `node` is empty, it is absurd. -/
+theorem Kind.IsEmpty.is_absurd (he : IsEmpty (.node r exs)) : ContainsSupOf exs r := by
+  cases he; assumption
+
+theorem Kind.IsEmpty.append (he1 : IsEmpty R1) (he2 : IsEmpty R2) : IsEmpty (R1 ++ R2) := by
+  induction R1 generalizing R2
+  case nil => simp_all
+  case cons x xs ih =>
+    rw [List.cons_append]
+    cases he1
+    apply! absurd _ (ih _ _)
+
+theorem Kind.IsEmpty.append_inv (he : IsEmpty (R1 ++ R2)) : IsEmpty R1 ∧ IsEmpty R2 := by
+  induction R1 generalizing R2
+  case nil => simp_all; apply empty
+  case cons x xs ih =>
+    rw [List.cons_append] at he
+    cases he
+    rename_i he1 he2
+    have ⟨_, _⟩ := ih he2
+    apply And.intro
+    . apply! absurd
+    . aesop
+
+end Capless
