Capless/Classifier/Subkind.lean
@@ -1,0 +1,14 @@
+import Capless.Classifier.Subtract
+
+namespace Capless
+
+/-- `K` is a subkind of `L` if every node in `K` is present in `L`. -/
+inductive Kind.Subkind : Kind -> Kind -> Prop where
+  | subtract : Subtract K1 K2 R -> IsEmpty R -> Subkind K1 K2
+
+theorem Kind.Subkind.empty_r_inv (hs : Subkind K1 K2) (he : IsEmpty K2) : IsEmpty K1 := by
+  cases hs
+  apply! Subtract.empty_r_inv
+
+
+end Capless
