Capless/Classifier/Subtract.lean
@@ -1,0 +1,560 @@
+import Capless.Classifier.Kind
+
+namespace Capless
+
+/-- This file defines the "subtraction" operation between two kind sets. -/
+
+inductive Subtree.Subtract : Subtree -> Subtree -> Kind -> Prop where
+  -- Basically we follow a few broad strokes:
+  -- - A \ (B \ C) = (A \ B) ∪ (A ∩ B ∩ C)
+  -- - For B of the form (.node r []) (no exclusion):
+  --   - If r < A, refine A
+  --   - If r > A, empty
+  --   - If r ⊥ A, A
+  -- Base case first
+  | tree : Subtract (.mk r1 ex1) (.mk r2 []) (.node r1 (r2 :: ex1))
+  -- Exclusion case
+  -- First, handle the cases where (B \ C) doesn't make sense
+  | excl_absurd_r :
+    r2.StrictSub a -> -- (B \ a) is just empty
+    Subtract (.mk r1 ex1) (.mk r2 (a :: ex2)) (.node r1 ex1)
+  | excl_irrelevant_r :
+    r2.Disjoint a -> -- (B \ a) = B
+    Subtract (.mk r1 ex1) (.mk r2 ex2) R ->
+    Subtract (.mk r1 ex1) (.mk r2 (a :: ex2)) R
+  -- Now, for cases where a is a subtree of r2
+  -- We use the formula A \ (B \ C) = (A \ B) ∪ (A ∩ B ∩ C)
+  | excl_subclass_r :
+    a.Subclass r2 ->
+    a.Subclass r1 -> -- A ∩ B ∩ C = a with all the exclusions
+    Subtract (.mk r1 ex1) (.mk r2 ex2) R ->
+    Subtract (.mk r1 ex1) (.mk r2 (a :: ex2)) ((.mk a ex1) :: R)
+                                        -- ^ we'd need (ex1 ++ ex2) here to be exact,
+                                        -- but if an element is in the ex2 subtree
+                                        -- and not already excluded from A, it is part
+                                        -- of (A \ B), so it's okay to keep anyway.
+  | excl_subclass_l :
+    a.Subclass r2 ->
+    r1.StrictSub a ->  -- B \ C excludes the entirety of A
+    Subtract (.mk r1 ex1) (.mk r2 (a :: ex2)) (.node r1 ex1)
+  | excl_irrelevant_l :
+    a.Subclass r2 ->
+    r1.Disjoint a -> -- irrelevant exclusion, A ∪ B ∪ C = empty
+    Subtract (.mk r1 ex1) (.mk r2 ex2) R ->
+    Subtract (.mk r1 ex1) (.mk r2 (a :: ex2)) R
+
+/-- Subtraction: `K.Subtract L` gives a Kind that contains all nodes in `K` but not in `L`. -/
+inductive Kind.Subtract : Kind -> Kind -> Kind -> Prop where
+  | empty_r : Subtract K .empty K
+  | union_r :
+    Subtract K [y] R1 ->
+    Subtract R1 (y' :: ys) R2 ->
+    Subtract K (y :: y' :: ys) R2
+  | empty_l : Subtract .empty [y] .empty
+  | union_l : x.Subtract y R1 -> Subtract xs [y] R2 -> Subtract (x::xs) [y] (R1 ++ R2)
+
+theorem Kind.Subtract.singleton (hs : x.Subtract y R) : Subtract [x] [y] R := by
+  have h := union_l hs .empty_l
+  simp at h
+  apply h
+
+theorem Kind.Subtract.is_singleton (hs : Subtract [x] [y] R) : x.Subtract y R := by
+  cases hs
+  case union_l ha hb => cases hb; simp_all
+
+theorem Subtree.Subtract.is_empty_l (hs : Subtract x y R) (hsc : Kind.IsEmpty [x]) : Kind.IsEmpty R := by
+  have hsc' := hsc.is_absurd
+  induction hs
+  case tree =>
+    apply Kind.IsEmpty.node
+    apply! ContainsSupOf.there
+  case excl_absurd_r => assumption
+  case excl_irrelevant_r ih => apply! ih
+  case excl_subclass_r hs2 hs1 hs ih =>
+    constructor
+    . apply hsc'.trans_subclass hs1
+    . apply! ih
+  case excl_subclass_l hs2 hss1 => apply! Kind.IsEmpty.node
+  case excl_irrelevant_l hd2 hd1 hs ih => apply! ih
+
+theorem Kind.Subtract.is_empty_l (hs : Subtract K1 K2 R) (he : IsEmpty K1) : IsEmpty R := by
+  induction hs
+  case empty_l => constructor
+  case union_l ha hb ih =>
+    cases he
+    apply! Kind.IsEmpty.append (ha.is_empty_l $ .node _) (ih _)
+  case empty_r => assumption
+  case union_r ha hb =>
+    apply hb
+    apply! ha
+
+theorem Kind.Subtract.empty_l' : Subtract [] K [] := by
+  induction K
+  case nil => apply empty_r
+  case cons x xs ih =>
+    cases xs
+    case nil => apply empty_l
+    case cons => apply union_r .empty_l ih
+
+theorem Kind.Subtract.absurd_l (hs : Subtract (.node r1 ex1) K R) (hsc : ContainsSupOf ex1 r1) : IsEmpty R := by
+  apply hs.is_empty_l
+  apply IsEmpty.node
+  assumption
+
+theorem Kind.Subtract.empty_l_inv (hs : Subtract [] K R) : R = [] := by
+  induction K generalizing R
+  case nil => cases hs; simp
+  case cons y ys ih =>
+    cases hs
+    case union_r ha hb => cases ha; apply! ih
+    case empty_l => simp
+
+theorem Subtree.Subtract.empty_implies_subclass
+  (hs : Subtract (.mk r1 ex1) (.mk r2 ex2) R)
+  (he : R.IsEmpty)
+  : ContainsSupOf ex1 r1 ∨ r1.Subclass r2 := by
+  cases hs
+  case tree =>
+    cases he.is_absurd <;> aesop
+  case excl_absurd_r => left; apply he.is_absurd
+  case excl_irrelevant_r hs => apply hs.empty_implies_subclass he
+  case excl_subclass_r hs =>
+    cases he
+    apply! hs.empty_implies_subclass
+  case excl_subclass_l => left; apply he.is_absurd
+  case excl_irrelevant_l hs => apply! hs.empty_implies_subclass
+
+theorem Subtree.Subtract.empty_r_inv (hs : Subtract S1 S2 R) (he : R.IsEmpty) (hsc2 : ContainsSupOf S2.excls S2.root) : ContainsSupOf S1.excls S1.root := by
+  induction hs
+  case tree => cases hsc2
+  case excl_absurd_r hss => apply he.is_absurd
+  case excl_irrelevant_r hd2 hs ih =>
+    cases hsc2
+    case here hs2 => cases hd2.not_subclass hs2
+    case there => apply! ih
+  case excl_subclass_r hs2 hs1 hs ih =>
+    cases he
+    rename_i he1 he2
+    cases hsc2
+    case here hsa =>
+      cases hs2.antisymm hsa
+      cases hs.empty_implies_subclass he2 <;> rename_i hs
+      . aesop
+      . cases hs1.antisymm hs; aesop
+    case there => apply! ih
+  case excl_subclass_l hs2 hss1 => apply he.is_absurd
+  case excl_irrelevant_l hs2 hd1 hs ih =>
+    cases hsc2
+    case here hsa =>
+      cases hs2.antisymm hsa
+      cases hs.empty_implies_subclass he <;> rename_i hs
+      . aesop
+      . cases hd1.not_subclass hs
+    case there => apply! ih
+
+theorem Kind.Subtract.empty_r_inv (hs : Subtract K1 K2 R) (he : IsEmpty R) (hek2 : IsEmpty K2) : IsEmpty K1 := by
+  induction hs
+  case empty_l => constructor
+  case union_l ha hb ih =>
+    have ⟨_, _⟩ := he.append_inv
+    apply! IsEmpty.append (.node $ ha.empty_r_inv _ hek2.is_absurd) (ih _ _)
+  case empty_r => assumption
+  case union_r ha hb =>
+    cases hek2
+    apply ha
+    . apply! hb
+    . apply! IsEmpty.node
+
+theorem Subtree.Subtract.exists' : ∃ R, Subtract (mk r1 ex1) (mk r2 ex2) R := by
+  induction ex2
+  case nil => exists .node r1 (r2 :: ex1); apply tree
+  case cons head tail ih =>
+    cases head.subclass_or_disjoint r2
+    case inl hs =>
+      have ⟨R, h⟩ := ih
+      cases head.subclass_or_disjoint r1
+      case inl hs1 =>
+        exists (.mk head ex1) :: R
+        apply! excl_subclass_r
+      case inr hs1 =>
+        cases hs1
+        case inl hs1 =>
+          exists .node r1 ex1
+          apply! excl_subclass_l
+        case inr hs1 =>
+          exists R
+          apply! excl_irrelevant_l _ hs1.symm
+    case inr hs =>
+      cases hs
+      case inl hs =>
+        exists .node r1 ex1
+        apply! excl_absurd_r
+      case inr hs =>
+        have ⟨R, h⟩ := ih
+        exists R
+        apply! excl_irrelevant_r hs.symm
+
+theorem Subtree.Subtract.exists (a b : Subtree) : ∃R, Subtract a b R := exists' (r1:=a.root) (ex1:= a.excls) (r2:=b.root) (ex2:=b.excls)
+
+theorem Kind.Subtract.exists' (a : Kind) (b : Subtree)  : ∃ R, Subtract a [b] R := by
+  induction a
+  case nil => exists .empty; apply empty_l
+  case cons x xs ih =>
+    have ⟨R1, h1⟩ := Subtree.Subtract.exists x b
+    have ⟨R2, h2⟩ := ih
+    exists R1 ++ R2
+    apply union_l h1 h2
+
+theorem Kind.Subtract.exists (a : Kind) (b: Kind) : ∃ R, Subtract a b R := by
+  induction b generalizing a
+  case nil => exists a; apply empty_r
+  case cons y ys ihb =>
+    cases ys
+    case nil => apply! exists'
+    case cons =>
+      have ⟨R1, h1⟩ := exists' a y
+      have ⟨R2, h2⟩ := ihb (a:=R1)
+      exists R2
+      apply union_r h1 h2
+
+theorem Subtree.Subtract.excl_absurd_r_inv
+  (hs : Subtract (mk r1 ex1) (mk r2 (a :: ex2)) R)
+  (hss : r2.StrictSub a)
+  : R = .node r1 ex1 := by
+  cases hs
+  case excl_absurd_r => rfl
+  case excl_irrelevant_r hd _ => cases hd.not_subclass hss.weaken
+  case excl_subclass_r h1 h2 _ => cases hss.antisymm h2
+  case excl_subclass_l h1 h2 => cases hss.antisymm h2
+  case excl_irrelevant_l h1 h2 _ => cases hss.antisymm h2
+
+theorem Subtree.Subtract.excl_irrelevant_r_inv
+  (hs : Subtract (mk r1 ex1) (mk r2 (a :: ex2)) R)
+  (hd : r2.Disjoint a)
+  : Subtract (mk r1 ex1) (mk r2 ex2) R := by
+  cases hs
+  case excl_absurd_r hss => cases hd.not_subclass hss.weaken
+  case excl_irrelevant_r => assumption
+  case excl_subclass_r hs1 hs2 hs => cases hd.symm.not_subclass hs2
+  case excl_subclass_l hs2 => cases hd.symm.not_subclass hs2
+  case excl_irrelevant_l hs2 _ => cases hd.symm.not_subclass hs2
+
+theorem Subtree.Subtract.excl_subclass_r_inv
+  (hs : Subtract (mk r1 ex1) (mk r2 (a :: ex2)) R)
+  (hs1 : a.Subclass r1)
+  (hs2 : a.Subclass r2)
+  : ∃ R', R = (mk a ex1) :: R' ∧ Subtract (mk r1 ex1) (mk r2 ex2) R' := by
+  cases hs
+  case excl_absurd_r hss => cases hss.antisymm hs2
+  case excl_irrelevant_r hd _ => cases hd.symm.not_subclass hs2
+  case excl_subclass_r => aesop
+  case excl_subclass_l hss _ => cases hss.antisymm hs1
+  case excl_irrelevant_l hd1 _ _ => cases hd1.symm.not_subclass hs1
+
+theorem Subtree.Subtract.excl_subclass_l_inv
+  (hs : Subtract (mk r1 ex1) (mk r2 (a :: ex2)) R)
+  (hs1 : r1.StrictSub a)
+  (hs2 : a.Subclass r2)
+  : R = .node r1 ex1 := by
+  cases hs
+  case excl_absurd_r hss => cases hss.antisymm hs2
+  case excl_irrelevant_r hd _ => cases hd.symm.not_subclass hs2
+  case excl_subclass_r => rename_i hsa _ _; cases hs1.antisymm hsa
+  case excl_subclass_l => rfl
+  case excl_irrelevant_l hd1 _ _ => cases hd1.not_subclass hs1.weaken
+
+theorem Subtree.Subtract.excl_irrelevant_l_inv
+  (hs : Subtract (mk r1 ex1) (mk r2 (a :: ex2)) R)
+  (hd1 : r1.Disjoint a)
+  (hs2 : a.Subclass r2)
+  : Subtract (mk r1 ex1) (mk r2 ex2) R := by
+  cases hs
+  case excl_absurd_r hss => cases hss.antisymm hs2
+  case excl_irrelevant_r hd _ => cases hd.symm.not_subclass hs2
+  case excl_subclass_r => rename_i hsa _ _; cases hd1.symm.not_subclass hsa
+  case excl_subclass_l => rename_i hss _; cases hd1.not_subclass hss.weaken
+  case excl_irrelevant_l => assumption
+
+theorem Subtree.Subtract.inj
+  (hs1 : Subtract a b R1)
+  (hs2 : Subtract a b R2)
+  : R1 = R2 := by
+  induction hs1 generalizing R2
+  case tree => cases hs2; simp
+  case excl_absurd_r hss => cases hs2.excl_absurd_r_inv hss; simp
+  case excl_irrelevant_r hd2 hs1 ih =>
+    apply ih
+    apply! hs2.excl_irrelevant_r_inv
+  case excl_subclass_r hsa2 hsa1 hs1 ih =>
+    have ⟨_, _, hs2'⟩ := hs2.excl_subclass_r_inv hsa1 hsa2
+    subst_vars
+    rw [List.cons_inj_right]
+    apply! ih
+  case excl_subclass_l hsa2 hss1 => cases hs2.excl_subclass_l_inv hss1 hsa2; simp
+  case excl_irrelevant_l hsa2 hd1 hs1 ih =>
+    apply ih
+    apply! hs2.excl_irrelevant_l_inv
+
+theorem Kind.Subtract.inj
+  (hs1 : Subtract K1 K2 R1)
+  (hs2 : Subtract K1 K2 R2)
+  : R1 = R2 := by
+  induction hs1 generalizing R2
+  case empty_r => cases hs2; simp
+  case union_r ha hb =>
+    cases hs2
+    rename_i hs2a hs2b
+    cases ha hs2a
+    apply hb hs2b
+  case empty_l => cases hs2; simp
+  case union_l ha hb ih =>
+    cases hs2
+    rename_i hs2a hs2b
+    cases ha.inj hs2a
+    cases ih hs2b
+    simp
+
+theorem Subtree.Subtract.is_empty_append_l
+  (hs1 : Subtract (mk r1 ex1) (mk r2 ex2) R1)
+  (he : R1.IsEmpty)
+  (hs2 : Subtract (mk r1 (a :: ex1)) (mk r2 ex2) R2)
+  : R2.IsEmpty := by
+  induction ex2 generalizing R1 R2
+  case nil =>
+    cases hs1
+    cases hs2
+    apply Kind.IsEmpty.node
+    cases he.is_absurd
+    case here => apply! ContainsSupOf.here
+    case there => apply! ContainsSupOf.there (.there _)
+  case cons a ex2 ih =>
+    cases hs1
+    case excl_absurd_r hss =>
+      apply hs2.is_empty_l
+      apply Kind.IsEmpty.node (.there he.is_absurd)
+    case excl_irrelevant_r hd2 hs1 => apply ih hs1 he; apply! excl_irrelevant_r_inv
+    case excl_subclass_r hsa1 hsa2 hs1 =>
+      cases he
+      rename_i he1 he2
+      have ⟨R, _, _⟩ := excl_subclass_r_inv hs2 hsa1 hsa2; subst_vars
+      constructor
+      . apply! ContainsSupOf.there
+      . apply! ih
+    case excl_subclass_l =>
+      apply hs2.is_empty_l
+      apply Kind.IsEmpty.node (.there he.is_absurd)
+    case excl_irrelevant_l hs1 => apply! ih hs1 _ (hs2.excl_irrelevant_l_inv _ _)
+
+theorem Subtree.Subtract.is_empty_swap_l
+  (hs1 : Subtract (mk r1 (a :: b :: ex1)) (mk r2 ex2) R1)
+  (he : R1.IsEmpty)
+  (hs2 : Subtract (mk r1 (b :: a :: ex1)) (mk r2 ex2) R2)
+  : R2.IsEmpty := by sorry
+
+theorem Subtree.Subtract.rfl
+  (hs : Subtract a a R)
+  : R.IsEmpty := by
+  cases hs
+  case tree => apply Kind.IsEmpty.node $ .here .rfl
+  case excl_absurd_r hss =>
+    apply Kind.IsEmpty.node $ .here hss.weaken
+  case excl_irrelevant_r r1 ex2 a hd hs =>
+    have ⟨R, h⟩ := Subtract.exists (mk r1 ex2) (mk r1 ex2)
+    apply h.is_empty_append_l h.rfl hs
+  case excl_subclass_r r1 ex2 _ _ _ hsa hs =>
+    have ⟨R, h⟩ := Subtract.exists (mk r1 ex2) (mk r1 ex2)
+    apply Kind.IsEmpty.absurd (.here .rfl)
+    apply h.is_empty_append_l h.rfl hs
+  case excl_subclass_l hss hs => cases hss.antisymm hs
+  case excl_irrelevant_l hd hs _ => cases hd.symm.not_subclass hs
+
+theorem Kind.Subtract.append_l'
+  (hs1 : Subtract K1 [y] R1)
+  (hs2 : Subtract K2 [y] R2)
+  : Subtract (K1 ++ K2) [y] (R1 ++ R2) := by
+  induction K1 generalizing K2 R1 R2
+  case nil => cases hs1; simp_all
+  case cons x xs ih =>
+    cases hs1
+    rename_i hs1a hs1b
+    rw [List.cons_append]
+    rw [List.append_assoc]
+    apply union_l hs1a
+    apply ih hs1b hs2
+
+theorem Kind.Subtract.append_l
+  (hs1 : Subtract K1 L R1)
+  (hs2 : Subtract K2 L R2)
+  : Subtract (K1 ++ K2) L (R1 ++ R2) := by
+  induction L generalizing K1 K2 R1 R2
+  case nil => cases hs1; cases hs2; apply empty_r
+  case cons y ys ih =>
+    cases ys
+    case nil => apply! append_l'
+    case cons =>
+      cases hs1
+      cases hs2
+      rename_i Ra hs1a hs1b Rb hs2a hs2b
+      apply union_r
+      apply append_l' hs1a hs2a
+      apply ih hs1b hs2b
+
+theorem Kind.Subtract.append_l_inv' (hs : Subtract (K1 ++ K2) [y] R) (hs1 : Subtract K1 [y] R1) : ∃ R2, R = R1 ++ R2 ∧ Subtract K2 [y] R2 := by
+  induction K1 generalizing K2 R R1
+  case nil => cases hs1; exists R
+  case cons x xs ih =>
+    cases hs1
+    rename_i hs1a hs1b
+    rw [List.cons_append] at hs
+    cases hs
+    rename_i hsa hsb
+    have ⟨R, heq, ih⟩ := ih hsb hs1b
+    cases hs1a.inj hsa
+    exists R
+    apply And.intro <;> simp_all
+
+theorem Kind.Subtract.append_l_inv (hs : Subtract (K1 ++ K2) L R) (hs1 : Subtract K1 L R1) : ∃ R2, R = R1 ++ R2 ∧ Subtract K2 L R2 := by
+  induction L generalizing K1 K2 R R1
+  generalize h : K1 ++ K2 = C at hs
+  case nil => cases hs1; cases hs; exists K2; apply And.intro; simp_all; apply empty_r
+  case cons y ys ih =>
+    cases ys
+    case nil => apply! append_l_inv'
+    case cons =>
+      cases hs1
+      rename_i hs1a hs1b
+      generalize h : K1 ++ K2 = C at hs
+      cases hs
+      rename_i hsa hsb
+      subst_vars
+      have ⟨R1, heq1, ih1⟩ := hsa.append_l_inv' hs1a
+      subst_vars
+      have ⟨R2, heq2, ih2⟩ := ih hsb hs1b
+      exists R2
+      simp_all
+      apply! union_r
+
+theorem Kind.Subtract.cons_l_inv (hs : Subtract (K :: K1) L R) (hs1 : Subtract [K] L R1) : ∃ R2, R = R1 ++ R2 ∧ Subtract K1 L R2 := by
+  apply append_l_inv hs hs1
+theorem Kind.Subtract.cons_l_inv' (hs : Subtract (x :: K1) [y] R) (hs1 : x.Subtract y R1) : ∃ R2, R = R1 ++ R2 ∧ Subtract K1 [y] R2 := by
+  have ⟨R, h1, h2⟩ := cons_l_inv hs (.union_l hs1 .empty_l)
+  simp at h1
+  aesop
+
+theorem Subtree.Subtract.is_empty_subroot_l
+  (hs1 : Subtract a b R1)
+  (he1 : R1.IsEmpty)
+  (hs2 : Subtract (mk c a.excls) b R2)
+  (hsub : c.Subclass a.root)
+  : R2.IsEmpty := by
+  induction hs1 generalizing R2
+  case tree =>
+    cases hs2; simp_all; apply Kind.IsEmpty.node
+    cases he1.is_absurd
+    case here hsub2 => apply ContainsSupOf.here $ hsub.trans hsub2
+    case there hsc => apply ContainsSupOf.there $ hsc.trans_subclass hsub
+  case excl_absurd_r hss =>
+    cases hs2.excl_absurd_r_inv hss
+    apply! Kind.IsEmpty.node $ he1.is_absurd.trans_subclass _
+  case excl_irrelevant_r hd hs1 ih =>
+    have hs2 := hs2.excl_irrelevant_r_inv hd
+    apply! ih
+  case excl_subclass_r a hsa2 hsa1 hs1 ih =>
+    simp_all
+    cases he1
+    cases Classifier.subclass_or_disjoint a c <;> rename_i hc
+    . have ⟨R, _, hs2⟩ := hs2.excl_subclass_r_inv hc hsa2
+      subst_vars
+      constructor; aesop
+      apply! ih
+    . cases hc <;> rename_i hc
+      . cases hs2.excl_subclass_l_inv hc hsa2
+        apply! Kind.IsEmpty.node (ContainsSupOf.trans_subclass _ hc.weaken)
+      . have hs2 := hs2.excl_irrelevant_l_inv hc.symm hsa2
+        apply! ih
+  case excl_subclass_l hsa2 hss1 =>
+    cases hs2.excl_subclass_l_inv (hss1.subclass_l hsub) hsa2
+    apply! Kind.IsEmpty.node $ he1.is_absurd.trans_subclass _
+  case excl_irrelevant_l hsa2 hd1 hs1 ih =>
+    have hs2 := hs2.excl_irrelevant_l_inv (hd1.refines_subclass_l hsub) hsa2
+    apply! ih
+
+theorem Subtree.Subtract.is_empty_middle
+  (hs1 : Subtract x y R1)
+  (he1 : R1.IsEmpty)
+  (hs2 : Subtract x z R2)
+  (hs3 : R2.Subtract [y] R3)
+  : R3.IsEmpty := by
+  induction hs2 generalizing R3
+  case tree => apply hs1.is_empty_append_l he1 hs3.is_singleton
+  case excl_absurd_r hss2 => cases hs1.inj hs3.is_singleton; simp_all
+  case excl_irrelevant_r hd2 hs2 ih => apply! ih
+  case excl_subclass_r r1 ex1 r2 ex2 _ a hsa2 hsa1 hs2 ih =>
+    have ⟨R0, h0⟩ := Subtract.exists (mk a ex1) y
+    have ⟨R', _, hs3'⟩ := hs3.cons_l_inv' h0
+    subst_vars
+    apply Kind.IsEmpty.append $ hs1.is_empty_subroot_l he1 h0 hsa1
+    apply! ih
+  case excl_subclass_l hsa2 hss1 => cases hs1.inj hs3.is_singleton; simp_all
+  case excl_irrelevant_l hsa2 hd1 hs2 ih => apply! ih
+
+theorem Kind.Subtract.is_empty_middle'
+  (hs1 : Subtract K [y] R1)
+  (he1 : R1.IsEmpty)
+  (hs2 : Subtract K [z] R2)
+  (hs3 : Subtract R2 [y] R3)
+  : R3.IsEmpty := by
+  induction K generalizing R1 R2 R3
+  case nil => cases hs1; cases hs2; cases hs3; simp_all
+  case cons x xs ih =>
+    cases hs1
+    cases hs2
+    rename_i hs1a hs1b R2 R1 hs2a hs2b
+    have ⟨he1a, he1b⟩ := he1.append_inv
+    have ⟨Rl, hl⟩ := Kind.Subtract.exists R1 [y]
+    have ⟨R3', _, hs3'⟩ := hs3.append_l_inv hl
+    subst_vars
+    apply IsEmpty.append
+    apply! hs1a.is_empty_middle
+    apply! ih
+
+mutual
+
+theorem Kind.Subtract.is_empty_swap_l
+  (hs1 : Subtract (.node r1 (a :: b :: ex1)) K R1)
+  (he1 : R1.IsEmpty)
+  (hs2 : Subtract (.node r1 (b :: a :: ex1)) K R2)
+  : R2.IsEmpty := by sorry
+
+theorem Kind.Subtract.is_empty_append_l
+  (hs1 : Subtract (.node r1 ex1) K R1)
+  (he1 : R1.IsEmpty)
+  (hs2 : Subtract (.node r1 (a :: ex1)) K R2)
+  : R2.IsEmpty := by
+  cases hs1
+  case empty_r => cases hs2; apply IsEmpty.node (.there he1.is_absurd)
+  case union_l ha hb => cases hb; simp_all; apply ha.is_empty_append_l he1 hs2.is_singleton
+  case union_r y' ys ha hb =>
+    cases hs2
+    rename_i ha2' hb2
+    have ha2 := ha2'.is_singleton
+    cases ha.is_singleton
+    case tree r2 =>
+      cases ha2
+      have ⟨R2', hb2'⟩ := Subtract.exists (node r1 (a :: r2 :: ex1)) (y' :: ys)
+      apply hb2'.is_empty_swap_l _ hb2
+      apply hb.is_empty_append_l he1 hb2'
+
+
+
+
+theorem Kind.Subtract.is_empty_subroot_l
+  (hs1 : Subtract (.node r1 ex1) K R1)
+  (he1 : R1.IsEmpty)
+  (hs2 : Subtract (.node c ex1) K R2)
+  (hsub : c.Subclass r1)
+  : R2.IsEmpty := sorry
+
+end
+
+end Capless
